WIP upto PCCUICConversion

pcuic/theories/PCUICClosedTyping.v
@@ -2,405 +2,11 @@
 From Coq Require Import Morphisms. 
 From MetaCoq.Template Require Import config utils.
 From MetaCoq.PCUIC Require Import PCUICAst PCUICAstUtils PCUICCases PCUICInduction
-     PCUICLiftSubst PCUICUnivSubst PCUICContextRelation PCUICTyping 
-     PCUICGlobalEnv PCUICWeakeningEnv PCUICSigmaCalculus.
+     PCUICLiftSubst PCUICUnivSubst PCUICContextRelation PCUICSigmaCalculus PCUICClosed 
+     PCUICOnFreeVars PCUICTyping PCUICReduction PCUICGlobalEnv PCUICWeakeningEnvConv PCUICWeakeningEnvTyp.
 
 Require Import ssreflect ssrbool.
 From Equations Require Import Equations.
-
-(** * Lemmas about the [closedn] predicate *)
-
-Lemma subst_instance_assumptions u ctx :
-  context_assumptions (subst_instance u ctx) = context_assumptions ctx.
-Proof.
-  induction ctx; cbnr.
-  destruct (decl_body a); cbn; now rewrite IHctx.
-Qed.
-#[global]
-Hint Rewrite subst_instance_assumptions : len.
-
-
-Lemma lift_decl_closed n k d : closed_decl k d -> lift_decl n k d = d.
-Proof.
-  case: d => na [body|] ty; rewrite /test_decl /lift_decl /map_decl /=; unf_term.
-  - move/andP => [cb cty]. now rewrite !lift_closed //.
-  - move=> cty; now rewrite !lift_closed //.
-Qed.
-
-Lemma closed_decl_upwards k d : closed_decl k d -> forall k', k <= k' -> closed_decl k' d.
-Proof.
-  case: d => na [body|] ty; rewrite /test_decl /=.
-  - move/andP => /= [cb cty] k' lek'. do 2 rewrite (@closed_upwards k) //.
-  - move=> cty k' lek'; rewrite (@closed_upwards k) //.
-Qed.
-
-Lemma alli_fold_context_k (p : nat -> context_decl -> bool) ctx f : 
-  (forall i d, p i d -> map_decl (f i) d = d) ->
-  alli p 0 (List.rev ctx) ->
-  fold_context_k f ctx = ctx.
-Proof.
-  intros Hf.
-  rewrite /fold_context_k /mapi.
-  generalize 0.
-  induction ctx using rev_ind; simpl; intros n; auto.
-  rewrite List.rev_app_distr /=.
-  move/andP=> [] Hc Hd.
-  rewrite Hf //; len. f_equal.
-  now apply IHctx.
-Qed.
-
-Lemma closedn_ctx_cons n d Γ : closedn_ctx n (d :: Γ) = closedn_ctx n Γ && closed_decl (n + #|Γ|) d.
-Proof.
-  rewrite /=. rewrite Nat.add_comm. bool_congr.
-Qed.
-
-Lemma test_context_k_app p n Γ Γ' :
-  test_context_k p n (Γ ,,, Γ') =
-  test_context_k p n Γ && test_context_k p (n + #|Γ|) Γ'.
-Proof.
-  rewrite /app_context /= !test_context_k_eq List.rev_app_distr alli_app /=. f_equal.
-  rewrite List.rev_length.
-  rewrite Nat.add_0_r alli_shift.
-  now setoid_rewrite Nat.add_assoc.
-Qed.
-
-Lemma closedn_ctx_app n Γ Γ' :
-  closedn_ctx n (Γ ,,, Γ') =
-  closedn_ctx n Γ && closedn_ctx (n + #|Γ|) Γ'.
-Proof.
-  now rewrite test_context_k_app.
-Qed.
-
-Lemma closed_ctx_lift n k ctx : closedn_ctx k ctx -> lift_context n k ctx = ctx.
-Proof.
-  induction ctx in n, k |- *; auto.
-  rewrite closedn_ctx_cons lift_context_snoc.
-  simpl.
-  move/andb_and => /= [Hctx Hd].
-  f_equal. rewrite IHctx // lift_decl_closed // Nat.add_comm //.
-Qed.
-
-Lemma map_decl_closed_ext (f : term -> term) g k (d : context_decl) : closed_decl k d -> 
-  (forall x, closedn k x -> f x = g x) -> 
-  map_decl f d = map_decl g d.
-Proof.
-  destruct d as [? [?|] ?] => /= cl Hfg;
-  unfold map_decl; simpl; f_equal.
-  rewrite Hfg => //. unfold closed_decl in cl.
-  simpl in cl. now move/andP: cl => []. 
-  move/andP: cl => [cl cl']. now rewrite Hfg.
-  now rewrite Hfg.
-Qed.
-
-Lemma test_decl_map_decl (p : term -> bool) (f : term -> term) d :
-  test_decl p (map_decl f d) = test_decl (p ∘ f) d.
-Proof.
-  rewrite /test_decl /map_decl; destruct d; simpl.
-  now destruct decl_body.
-Qed.
-
-Lemma plus_minus' n m : n + m - m = n.
-Proof. lia. Qed.
-
-Lemma test_context_k_mapi (p : nat -> term -> bool) k (f : nat -> term -> term) ctx :
-  test_context_k p k (mapi_context f ctx) =
-  test_context_k (fun i t => p i (f (i - k) t)) k ctx.
-Proof.
-  induction ctx; simpl; auto.
-  rewrite IHctx. f_equal. rewrite test_decl_map_decl.
-  len. now setoid_rewrite plus_minus'.
-Qed.
-#[global]
-Hint Rewrite test_context_k_mapi : map.
-
-Lemma test_context_k_map (p : nat -> term -> bool) k (f : term -> term) ctx :
-  test_context_k p k (map_context f ctx) =
-  test_context_k (fun i t => p i (f t)) k ctx.
-Proof.
-  induction ctx; simpl; auto.
-  rewrite IHctx. f_equal. rewrite test_decl_map_decl.
-  now len.
-Qed.
-#[global]
-Hint Rewrite test_context_k_map : map.
-
-Lemma closedn_lift n k k' t : closedn k t -> closedn (k + n) (lift n k' t).
-Proof.
-  revert k.
-  induction t in n, k' |- * using term_forall_list_ind; intros;
-    simpl in *; rewrite -> ?andb_and in *;
-    autorewrite with map;
-    simpl closed in *; solve_all;
-    unfold test_def, test_snd, test_predicate_k, test_branch_k in *;
-      try solve [simpl lift; simpl closed; f_equal; auto; repeat (rtoProp; simpl in *; solve_all)]; try easy.
-
-  - elim (Nat.leb_spec k' n0); intros. simpl.
-    elim (Nat.ltb_spec); auto. apply Nat.ltb_lt in H. lia.
-    simpl. elim (Nat.ltb_spec); auto. intros.
-    apply Nat.ltb_lt in H. lia.
-Qed.
-
-Lemma closedn_lift_inv n k k' t : k <= k' ->
-                                   closedn (k' + n) (lift n k t) ->
-                                   closedn k' t.
-Proof.
-  induction t in n, k, k' |- * using term_forall_list_ind; intros;
-    simpl in *;
-    autorewrite with map;
-    simpl closed in *; repeat (rtoProp; simpl in *; solve_all); try change_Sk;
-    unfold test_def, test_predicate_k, test_branch_k, shiftf in *; 
-    rewrite -> ?map_length, ?Nat.add_assoc in *;
-    simpl in *; eauto 2 with all.
-
-  - revert H0.
-    elim (Nat.leb_spec k n0); intros. simpl in *.
-    elim (Nat.ltb_spec); auto. apply Nat.ltb_lt in H1. intros. lia.
-    revert H1. simpl. elim (Nat.ltb_spec); auto. intros. apply Nat.ltb_lt. lia.
-  - specialize (IHt2 n (S k) (S k')). eauto with all.
-  - specialize (IHt2 n (S k) (S k')). eauto with all.
-  - specialize (IHt3 n (S k) (S k')). eauto with all.
-  - rtoProp. solve_all; unfold shiftf in *.
-    * now len in H6.
-    * eapply (i n (#|pcontext p| + k)). lia.
-      now len in H3.
-  - rtoProp. solve_all; unfold shiftf in *.
-    * now len in H7.
-    * eapply (b0 n (#|bcontext x| + k)); eauto; try lia.
-  - rtoProp. solve_all. specialize (b0 n (#|m| + k) (#|m| + k')).
-    now len in H1.
-  - rtoProp. solve_all. specialize (b0 n (#|m| + k) (#|m| + k')). eauto with all.
-Qed.
-
-Lemma closedn_mkApps k f u:
-  closedn k (mkApps f u) = closedn k f && forallb (closedn k) u.
-Proof.
-  induction u in k, f |- *; simpl; auto.
-  - now rewrite andb_true_r.
-  - now rewrite IHu /= andb_assoc.
-Qed.
-
-#[global] Remove Hints absurd_eq_true trans_eq_bool f_equal2_nat f_equal_nat : core.
-
-Lemma closedn_subst_eq s k k' t :
-  forallb (closedn k) s -> 
-  closedn (k + k' + #|s|) t =
-  closedn (k + k') (subst s k' t).
-Proof.
-  intros Hs. solve_all. revert Hs.
-  induction t in k' |- * using term_forall_list_ind; intros;
-    simpl in *;
-    autorewrite with map => //;
-    simpl closed in *; try change_Sk;
-    unfold test_def, test_branch_k, test_predicate_k in *; simpl in *;
-    solve_all.
-
-  - elim (Nat.leb_spec k' n); intros. simpl.
-    destruct nth_error eqn:Heq.
-    -- rewrite closedn_lift.
-       now eapply nth_error_all in Heq; simpl; eauto; simpl in *.
-       eapply nth_error_Some_length in Heq.
-       eapply Nat.ltb_lt. lia.
-    -- simpl. elim (Nat.ltb_spec); auto. intros.
-       apply nth_error_None in Heq. symmetry. apply Nat.ltb_lt. lia.
-       apply nth_error_None in Heq. intros. symmetry. eapply Nat.ltb_nlt.
-       intros H'. lia.
-    -- simpl.
-      elim: Nat.ltb_spec; symmetry. apply Nat.ltb_lt. lia.
-      apply Nat.ltb_nlt. intro. lia.
-
-  - specialize (IHt2 (S k')).
-    rewrite <- Nat.add_succ_comm in IHt2.
-    rewrite IHt1 // IHt2 //.
-  - specialize (IHt2 (S k')).
-    rewrite <- Nat.add_succ_comm in IHt2.
-    rewrite IHt1 // IHt2 //.
-  - specialize (IHt3 (S k')).
-    rewrite <- Nat.add_succ_comm in IHt3.
-    rewrite IHt1 // IHt2 // IHt3 //.
-  - rewrite IHt //.
-    f_equal; [|solve_all;f_equal]. f_equal. f_equal. f_equal.
-    all:len; solve_all.
-    * specialize (e (#|pcontext p| + k')).
-      now rewrite Nat.add_assoc (Nat.add_comm k) in e.
-    * specialize (b (#|bcontext x| + k')).
-      now rewrite Nat.add_assoc (Nat.add_comm k) in b.
-  - rewrite a //.
-    specialize (b (#|m| + k')).
-    rewrite Nat.add_assoc in b.
-    rewrite (Nat.add_comm k #|m|) in b. 
-    rewrite b //.
-  - rewrite a //.
-    specialize (b (#|m| + k')).
-    rewrite Nat.add_assoc in b.
-    rewrite (Nat.add_comm k #|m|) in b. 
-    rewrite b //.
-Qed.
-
-Lemma closedn_subst_eq' s k k' t :
-  closedn (k + k') (subst s k' t) ->
-  closedn (k + k' + #|s|) t.
-Proof.
-  intros Hs. solve_all. revert Hs.
-  induction t in k' |- * using term_forall_list_ind; intros;
-    simpl in *;
-    autorewrite with map;
-    simpl closed in *; repeat (rtoProp; f_equal; solve_all);  try change_Sk;
-    unfold test_def, map_branch, test_branch, test_predicate in *; simpl in *; eauto 4 with all.
-
-  - move: Hs; elim (Nat.leb_spec k' n); intros. simpl.
-    destruct nth_error eqn:Heq.
-    -- eapply Nat.ltb_lt.
-       eapply nth_error_Some_length in Heq. lia.
-    -- simpl. simpl in Hs.
-       apply nth_error_None in Heq. apply Nat.ltb_lt.
-       apply Nat.ltb_lt in Hs; lia.
-    -- simpl in Hs. eapply Nat.ltb_lt in Hs.
-       apply Nat.ltb_lt. lia.
-
-  - specialize (IHt2 (S k')).
-    rewrite <- Nat.add_succ_comm in IHt2. eauto.
-  - specialize (IHt2 (S k')).
-    rewrite <- Nat.add_succ_comm in IHt2. eauto.
-  - specialize (IHt3 (S k')).
-    rewrite <- Nat.add_succ_comm in IHt3. eauto.
-  - move/andb_and: H => [hpar hret].
-    rewrite !Nat.add_assoc in hret.
-    specialize (i (#|pcontext p| + k')).
-    rewrite Nat.add_assoc (Nat.add_comm k) in i.
-    simpl in *.  unfold test_predicate_k. simpl. solve_all.
-    * now len in H5.
-  - unfold test_branch_k in *. rtoProp; solve_all.
-    * cbn in H4. now len in H4.
-    * specialize (b0 (#|bcontext x| + k')).
-      rewrite Nat.add_assoc (Nat.add_comm k) in b0.
-      simpl in H2. len in H2. rewrite !Nat.add_assoc in H2. eauto.
-  - move/andP: b => [hty hbod]. rewrite a0 //.
-    specialize (b0 (#|m| + k')).
-    rewrite Nat.add_assoc (Nat.add_comm k #|m|) in b0. 
-    rewrite b0 //. now autorewrite with len in hbod.
-  - move/andP: b => [hty hbod]. rewrite a0 //.
-    specialize (b0 (#|m| + k')).
-    rewrite Nat.add_assoc (Nat.add_comm k #|m|) in b0. 
-    rewrite b0 //. now autorewrite with len in hbod.
-Qed.
-
-Lemma closedn_subst s k k' t :
-  forallb (closedn k) s -> 
-  closedn (k + k' + #|s|) t ->
-  closedn (k + k') (subst s k' t).
-Proof.
-  intros; now rewrite -closedn_subst_eq.
-Qed.
-
-Lemma closedn_subst0 s k t :
-  forallb (closedn k) s -> closedn (k + #|s|) t ->
-  closedn k (subst0 s t).
-Proof.
-  intros.
-  generalize (closedn_subst s k 0 t H).
-  rewrite Nat.add_0_r. eauto.
-Qed.
-
-Lemma subst_closedn s k t : closedn k t -> subst s k t = t.
-Proof.
-  intros Hcl.
-  pose proof (simpl_subst_rec t s 0 k k).
-  intros. assert(Hl:=lift_closed (#|s| + 0) _ _ Hcl).
-  do 2 (forward H; auto). rewrite Hl in H.
-  rewrite H. now apply lift_closed.
-Qed.
-
-Lemma closedn_subst_instance k t u :
-  closedn k (subst_instance u t) = closedn k t.
-Proof.
-  revert k.
-  induction t in |- * using term_forall_list_ind; intros;
-    simpl in *; rewrite -> ?andb_and in *;
-    autorewrite with map; len;
-    unfold test_predicate_k, test_branch_k in *; solve_all.
-
-  - unfold test_predicate_k, map_predicate; simpl.
-    f_equal. f_equal. f_equal. f_equal.
-    all: len; solve_all.
-  - unfold test_def, map_def. simpl.
-    do 3 (f_equal; intuition eauto).
-  - unfold test_def, map_def. simpl.
-    do 3 (f_equal; intuition eauto).
-Qed.
-
-Lemma closed_map_subst_instance n u l : 
-  forallb (closedn n) (map (subst_instance u) l) = 
-  forallb (closedn n) l.
-Proof.
-  induction l; simpl; auto.
-  now rewrite closedn_subst_instance IHl.
-Qed.
-
-Lemma closedn_ctx_tip n d : closedn_ctx n [d] = closed_decl n d.
-Proof. now rewrite test_context_k_eq /= andb_true_r Nat.add_0_r. Qed.
-
-Lemma closedn_All_local_closed:
-  forall (cf : checker_flags) (Σ : global_env_ext) (Γ : context) (ctx : list context_decl)
-         (wfΓ' : wf_local Σ (Γ ,,, ctx)),
-    All_local_env_over typing
-    (fun (Σ0 : global_env_ext) (Γ0 : context) (_ : wf_local Σ0 Γ0) (t T : term) (_ : Σ0;;; Γ0 |- t : T) =>
-       closedn #|Γ0| t && closedn #|Γ0| T) Σ (Γ ,,, ctx) wfΓ' ->
-    closedn_ctx 0 Γ && closedn_ctx #|Γ| ctx.
-Proof.
-  intros cf Σ Γ ctx wfΓ' al.
-  remember (Γ ,,, ctx) as Γ'. revert Γ' wfΓ' ctx HeqΓ' al.
-  induction Γ. simpl. intros. subst. unfold app_context in *. rewrite app_nil_r in wfΓ' al.
-  induction al; try constructor;
-  rewrite closedn_ctx_cons /=; cbn.
-  move/andP: p => [] /= -> _. now rewrite IHal.
-  now rewrite IHal /= /test_decl /=.
-  intros.
-  unfold app_context in *. subst Γ'.
-  specialize (IHΓ (ctx ++ a :: Γ) wfΓ' (ctx ++ [a])).
-  rewrite -app_assoc in IHΓ. specialize (IHΓ eq_refl al).
-  rewrite closedn_ctx_app /= Nat.add_1_r andb_assoc in IHΓ.
-  now rewrite closedn_ctx_cons /=.
-Qed.
-
-Lemma closedn_mkProd_or_LetIn n d T :
-    closed_decl n d && closedn (S n) T = closedn n (mkProd_or_LetIn d T).
-Proof.
-  destruct d as [na [b|] ty]; reflexivity.
-Qed.
-
-Lemma closedn_mkLambda_or_LetIn (Γ : context) d T :
-    closed_decl #|Γ| d ->
-    closedn (S #|Γ|) T -> closedn #|Γ| (mkLambda_or_LetIn d T).
-Proof.
-  destruct d as [na [b|] ty]; simpl in *. unfold closed_decl.
-  simpl. now move/andP => [] /= -> ->.
-  simpl. now move/andP => [] /= _ -> ->.
-Qed.
-
-Lemma closedn_it_mkProd_or_LetIn n (ctx : list context_decl) T :
-  closedn n (it_mkProd_or_LetIn ctx T) = 
-  closedn_ctx n ctx && closedn (n + #|ctx|) T.
-Proof.
-  induction ctx in n, T |- *. simpl.
-  - now rewrite Nat.add_0_r.
-  - rewrite closedn_ctx_cons.
-    rewrite (IHctx n (mkProd_or_LetIn a T)) /= -closedn_mkProd_or_LetIn.
-    now rewrite // plus_n_Sm andb_assoc.
-Qed.
-
-Lemma closedn_it_mkLambda_or_LetIn
-      (Γ : context) (ctx : list context_decl) T :
-    closedn_ctx #|Γ| ctx ->
-    closedn (#|Γ| + #|ctx|) T -> closedn #|Γ| (it_mkLambda_or_LetIn ctx T).
-Proof.
-  induction ctx in Γ, T |- *. simpl.
-  - now rewrite Nat.add_0_r.
-  - rewrite closedn_ctx_cons; move/andP => [] cctx ca cT.
-    apply (IHctx Γ (mkLambda_or_LetIn a T) cctx).
-    simpl in cT. rewrite <- app_length.
-    eapply closedn_mkLambda_or_LetIn;
-      now rewrite app_length // plus_n_Sm.
-Qed.
 
 Lemma type_local_ctx_All_local_env {cf:checker_flags} P Σ Γ Δ s : 
   All_local_env (lift_typing P Σ) Γ ->
@@ -424,10 +30,6 @@ Proof.
   destruct s => //. destruct wfctx; eauto.
   destruct s => //. destruct wfctx. exists t; auto.
 Qed.
-
-Definition Pclosed :=
-  (fun (_ : global_env_ext) (Γ : context) (t T : term) =>
-           closedn #|Γ| t && closedn #|Γ| T).
 
 Lemma type_local_ctx_Pclosed Σ Γ Δ s :
   type_local_ctx (lift_typing Pclosed) Σ Γ Δ s ->
@@ -480,106 +82,11 @@ Proof.
     unfold closed_decl. unfold Pclosed, lift_typing in *. now simpl.
 Qed.
 
-Lemma closed_subst_context n (Δ Δ' : context) t :
-  closedn (n + #|Δ|) t ->
-  Alli (fun i d => closed_decl (n + S #|Δ| + i) d) 0 (List.rev Δ') -> 
-  Alli (fun i d => closed_decl (n + #|Δ| + i) d) 0 (List.rev (subst_context [t] 0 Δ')).
-Proof.
-  induction Δ' in Δ |- *.
-  intros. simpl. auto. constructor.
-  destruct a as [? [] ?]; simpl.
-  - intros. eapply Alli_app in X as [X X'].
-    rewrite subst_context_snoc. simpl. eapply Alli_app_inv.
-    eapply IHΔ'; eauto. constructor; [|constructor].
-    simpl. 
-    rewrite /test_decl /map_decl /= Nat.add_0_r List.rev_length subst_context_length.
-    inv X'. unfold test_decl in H0. simpl in H0.
-    rewrite List.rev_length Nat.add_0_r in H0.
-    move/andP: H0 => [Hl Hr];
-    rewrite !closedn_subst /= ?H //; eapply closed_upwards; eauto; try lia.
-  - intros. eapply Alli_app in X as [X X'].
-    rewrite subst_context_snoc. simpl. eapply Alli_app_inv.
-    eapply IHΔ'; eauto. constructor; [|constructor].
-    simpl. 
-    rewrite /test_decl /map_decl /= Nat.add_0_r List.rev_length subst_context_length.
-    inv X'. unfold test_decl in H0. simpl in H0.
-    rewrite List.rev_length Nat.add_0_r in H0.
-    rewrite !closedn_subst /= ?H //; eapply closed_upwards; eauto; try lia.
-Qed.
-
-Lemma closed_smash_context_gen n (Δ Δ' : context) :
-  Alli (fun i d => closed_decl (n + i) d) 0 (List.rev Δ) -> 
-  Alli (fun i d => closed_decl (n + #|Δ| + i) d) 0 (List.rev Δ') -> 
-  Alli (fun i d => closed_decl (n + i) d) 0 (List.rev (smash_context Δ' Δ)).
-Proof.
-  induction Δ in Δ' |- *.
-  intros. simpl. auto.
-  simpl. eapply (Alli_impl _ X0). simpl. now rewrite Nat.add_0_r.
-  destruct a as [? [] ?]; simpl.
-  - intros. eapply Alli_app in X as [X X'].
-    eapply IHΔ; eauto.
-    inv X'. unfold closed_decl in H. simpl in H.
-    rewrite List.rev_length Nat.add_0_r in H.
-    clear X1. eapply closed_subst_context; auto.
-    now move/andP: H => [].
-  - intros. eapply Alli_app in X as [X X'].
-    eapply IHΔ; eauto.
-    inv X'. unfold closed_decl in H. simpl in H.
-    rewrite List.rev_length Nat.add_0_r in H.
-    clear X1. rewrite List.rev_app_distr.
-    eapply Alli_app_inv; repeat constructor.
-    now rewrite Nat.add_0_r /=.
-    rewrite List.rev_length /=. clear -X0.
-    apply Alli_shift, (Alli_impl _ X0). intros.
-    eapply closed_decl_upwards; eauto; lia.
-Qed.
-
-Lemma closed_smash_context_unfold n (Δ : context) :
-  Alli (fun i d => closed_decl (n + i) d) 0 (List.rev Δ) -> 
-  Alli (fun i d => closed_decl (n + i) d) 0 (List.rev (smash_context [] Δ)).
-Proof.
-  intros; apply (closed_smash_context_gen n _ []); auto. constructor.
-Qed.
-
-Lemma closedn_subst_instance_context {k Γ u} :
-  closedn_ctx k (subst_instance u Γ) = closedn_ctx k Γ.
-Proof.
-  rewrite !test_context_k_eq.
-  rewrite rev_subst_instance.
-  rewrite alli_map.
-  apply alli_ext; intros i [? [] ?]; unfold closed_decl, test_decl; cbn.
-  all: now rewrite !closedn_subst_instance.
-Qed.
-
-Lemma closedn_ctx_spec k Γ : closedn_ctx k Γ <~> Alli (fun k => closed_decl k) k (List.rev Γ).
-Proof.
-  split.
-  - induction Γ as [|d ?].
-    + constructor.
-    + rewrite closedn_ctx_cons => /andP [clΓ cld].
-      simpl in *. eapply Alli_app_inv; simpl; eauto.
-      repeat constructor. now rewrite List.rev_length.
-  - induction Γ in k |- * => //.
-    simpl. move/Alli_app => [clΓ cld].
-    simpl. depelim cld. rewrite List.rev_length in i.
-    now rewrite i IHΓ.
-Qed.
-
-Lemma closedn_smash_context (Γ : context) n :
-  closedn_ctx n Γ ->
-  closedn_ctx n (smash_context [] Γ).
-Proof.
-  intros.
-  epose proof (closed_smash_context_unfold n Γ).
-  apply closedn_ctx_spec. rewrite -(Nat.add_0_r n). apply Alli_shiftn, X.
-  apply closedn_ctx_spec in H. rewrite -(Nat.add_0_r n) in H.
-  now apply (Alli_shiftn_inv 0 _ n) in H.
-Qed.
-
 Lemma weaken_env_prop_closed {cf:checker_flags} : 
   weaken_env_prop (lift_typing (fun (_ : global_env_ext) (Γ : context) (t T : term) =>
   closedn #|Γ| t && closedn #|Γ| T)).
 Proof. repeat red. intros. destruct t; red in X0; eauto. Qed.
+
 
 Lemma declared_projection_closed_ind {cf:checker_flags} {Σ : global_env} {wfΣ : wf Σ}{mdecl idecl cdecl p pdecl} : 
   declared_projection Σ p mdecl idecl cdecl pdecl ->
@@ -591,7 +98,7 @@ Proof.
   intros isdecl X0.
   pose proof (declared_projection_inv weaken_env_prop_closed wfΣ X0 isdecl) as onp.
   set (declared_inductive_inv _ wfΣ X0 _) as oib in *.
-  clearbody oib.
+  clearbody oib. unfold declared_projection in isdecl.
   have onpars := onParams (declared_minductive_inv weaken_env_prop_closed wfΣ X0 isdecl.p1.p1).
   have parslen := onNpars (declared_minductive_inv weaken_env_prop_closed wfΣ X0 isdecl.p1.p1).
   simpl in onp.
@@ -643,6 +150,7 @@ Proof.
   rewrite context_assumptions_app in Heq'. lia.
 Qed.
 
+
 Lemma closedn_ctx_alpha {k ctx ctx'} : 
   All2 (PCUICEquality.compare_decls eq eq) ctx ctx' ->
   closedn_ctx k ctx = closedn_ctx k ctx'.
@@ -652,23 +160,6 @@ Proof.
   rewrite (All2_length X).
   destruct r; cbn; now subst.
 Qed.
-
-Definition closed_constructor_body mdecl (b : constructor_body) :=
-  closedn_ctx (#|ind_bodies mdecl| + #|ind_params mdecl|) b.(cstr_args) &&
-  forallb (closedn (#|ind_bodies mdecl| + #|ind_params mdecl| + #|b.(cstr_args)|)) b.(cstr_indices) &&
-  closedn #|ind_bodies mdecl| b.(cstr_type).
-
-Definition closed_inductive_body mdecl idecl :=
-  closedn 0 idecl.(ind_type) &&
-  closedn_ctx #|mdecl.(ind_params)| idecl.(ind_indices) &&
-  forallb (closed_constructor_body mdecl) idecl.(ind_ctors) &&
-  forallb (fun x => closedn (S (ind_npars mdecl)) x.2) idecl.(ind_projs).
-
-Definition closed_inductive_decl mdecl :=
-  closed_ctx (ind_params mdecl) &&
-  forallb (closed_inductive_body mdecl) (ind_bodies mdecl).
-
-Set SimplIsCbn.
 
 Lemma on_global_env_impl `{checker_flags} Σ P Q :
   (forall Σ Γ t T, on_global_env P Σ.1 -> P Σ Γ t T -> Q Σ Γ t T) ->
@@ -714,6 +205,7 @@ Proof.
        intros. now apply X.
 Qed.
 
+
 Lemma declared_decl_closed_ind `{checker_flags} {Σ : global_env} {wfΣ : wf Σ} {cst decl} :
   lookup_env Σ cst = Some decl ->
   Forall_decls_typing (fun (_ : global_env_ext) (Γ : context) (t T : term) => closedn #|Γ| t && closedn #|Γ| T) Σ ->
@@ -726,26 +218,7 @@ Proof.
   red; intros. unfold lift_typing in *. destruct T; intuition auto with wf.
   destruct X1 as [s0 Hs0]. simpl. rtoProp; intuition.
 Qed.
-
-Lemma closedn_mapi_rec_ext (f g : nat -> context_decl -> context_decl) (l : context) n k' :
-  closedn_ctx k' l ->
-  (forall k x, n <= k -> k < length l + n -> 
-    closed_decl (k' + #|l|) x ->
-    f k x = g k x) ->
-  mapi_rec f l n = mapi_rec g l n.
-Proof.
-  intros cl Hfg.
-  induction l in n, cl, Hfg |- *; simpl; try congruence.
-  intros. rewrite Hfg; simpl; try lia.
-  rewrite closedn_ctx_cons in cl.
-  move/andP: cl => [cll clr]. eapply closed_decl_upwards; eauto. lia.
-  f_equal.
-  rewrite IHl; auto.
-  rewrite closedn_ctx_cons in cl.
-  now move/andP: cl => [].
-  intros. apply Hfg. simpl; lia. simpl. lia. simpl.
-  eapply closed_decl_upwards; eauto. lia.
-Qed.
+ 
 
 Lemma closedn_All_local_env (ctx : list context_decl) :
   All_local_env 
@@ -755,6 +228,7 @@ Lemma closedn_All_local_env (ctx : list context_decl) :
 Proof.
   induction 1; auto; rewrite closedn_ctx_cons IHX /=; now move/andP: t0 => [].
 Qed.
+
 
 Lemma declared_minductive_closed_ind {cf:checker_flags} {Σ : global_env} {wfΣ : wf Σ}{mdecl mind} : 
   Forall_decls_typing
@@ -821,329 +295,6 @@ Proof.
     now eapply declared_projection_closed_ind in H.
 Qed.
 
-Lemma closed_declared_ind {Σ ind mdecl idecl} : 
-  declared_inductive Σ ind mdecl idecl ->
-  closed_inductive_decl mdecl ->
-  closed_inductive_body mdecl idecl.
-Proof.
-  intros [decli hnth] [clpars clbods]%andb_and.
-  solve_all.
-  now eapply nth_error_all in clbods; eauto.
-Qed.
-
-
-Lemma closedn_ctx_decl {Γ n d k} :
-  closedn_ctx k Γ ->
-  nth_error Γ n = Some d ->
-  closed_decl (k + #|Γ| - S n) d.
-Proof.
-  intros clΓ hnth. eapply closedn_ctx_spec in clΓ.
-  pose proof (nth_error_Some_length hnth).
-  rewrite (nth_error_rev _ _ H) in hnth.
-  eapply nth_error_alli in clΓ; eauto.
-  simpl in clΓ. eapply closed_decl_upwards; eauto. lia.
-Qed.
-
-Arguments lift_context _ _ _ : simpl never. 
-Arguments subst_context _ _ _ : simpl never.
-
-Lemma closedn_ctx_lift n k k' Γ : closedn_ctx k Γ ->
-  closedn_ctx (n + k) (lift_context n k' Γ).
-Proof.
-  induction Γ as [|d ?]; cbn; auto; rewrite lift_context_snoc !closedn_ctx_cons /=;
-    move/andP=> [clΓ cld]; rewrite IHΓ //;
-  autorewrite with len in cld.
-  move: cld; rewrite /test_decl. simpl.
-  move/andP=> [clb clt]; apply andb_and; split.
-  destruct (decl_body d) => /= //. simpl in clb |- *.
-  eapply (closedn_lift n) in clb.
-  autorewrite with len. now rewrite Nat.add_comm (Nat.add_comm n) Nat.add_assoc.
-  eapply (closedn_lift n) in clt.
-  autorewrite with len. now rewrite Nat.add_comm (Nat.add_comm n) Nat.add_assoc.
-Qed.
-
-Lemma closedn_ctx_subst k k' s Γ : 
-  closedn_ctx (k + k' + #|s|) Γ ->
-  forallb (closedn k) s ->
-  closedn_ctx (k + k') (subst_context s k' Γ).
-Proof.
-  induction Γ as [|d ?] in k' |- *; auto; rewrite subst_context_snoc !closedn_ctx_cons /=;
-  move/andP=> [clΓ cld]  cls; rewrite IHΓ //;
-  autorewrite with len in cld.
-  move: cld; rewrite /test_decl. simpl.
-  move/andP=> [clb clt]; apply andb_and; split.
-  destruct (decl_body d) => /= //. simpl in clb |- *.
-  rewrite -Nat.add_assoc [#|s| + _]Nat.add_comm Nat.add_assoc in clb.
-  rewrite -(Nat.add_assoc k) in clb.
-  eapply (closedn_subst s) in clb => //. rewrite Nat.add_assoc in clb.
-  autorewrite with len. now rewrite (Nat.add_comm #|Γ|).
-  rewrite -Nat.add_assoc [#|s| + _]Nat.add_comm Nat.add_assoc in clt.
-  rewrite -(Nat.add_assoc k) in clt.
-  eapply (closedn_subst s) in clt => //. rewrite Nat.add_assoc in clt.
-  autorewrite with len. now rewrite (Nat.add_comm #|Γ|).
-Qed.
-
-Lemma map_subst_closedn (s : list term) (k : nat) l :
-  forallb (closedn k) l -> map (subst s k) l = l.
-Proof.
-  induction l; simpl; auto.
-  move/andP=> [cla cll]. rewrite IHl //.
-  now rewrite subst_closedn.
-Qed.
-
-Lemma closedn_extended_subst_gen Γ k k' : 
-  closedn_ctx k Γ -> 
-  forallb (closedn (k' + k + context_assumptions Γ)) (extended_subst Γ k').
-Proof.
-  induction Γ as [|[? [] ?] ?] in k, k' |- *; auto; rewrite ?closedn_ctx_cons /=;
-   move/andP => [clΓ /andP[clb clt]].
-  - rewrite IHΓ //.
-    epose proof (closedn_subst (extended_subst Γ k') (k' + k + context_assumptions Γ) 0).
-    autorewrite with len in H. rewrite andb_true_r.
-    eapply H; auto.
-    replace (k' + k + context_assumptions Γ + #|Γ|)
-    with (k + #|Γ| + (context_assumptions Γ + k')) by lia.
-    eapply closedn_lift. eapply clb.
-  - apply andb_and. split.
-    * apply Nat.ltb_lt; lia.
-    * specialize (IHΓ k (S k') clΓ).
-      red. rewrite -IHΓ. f_equal. f_equal. lia.
-Qed.
-
-Lemma closedn_extended_subst Γ : 
-  closed_ctx Γ -> 
-  forallb (closedn (context_assumptions Γ)) (extended_subst Γ 0).
-Proof.
-  intros clΓ. now apply (closedn_extended_subst_gen Γ 0 0).
-Qed.
-
-Lemma closedn_ctx_expand_lets k Γ Δ :
-  closedn_ctx k Γ ->
-  closedn_ctx (k + #|Γ|) Δ ->
-  closedn_ctx (k + context_assumptions Γ) (expand_lets_ctx Γ Δ).
-Proof.
-  intros clΓ clΔ.
-  rewrite /expand_lets_ctx /expand_lets_k_ctx.
-  rewrite -(Nat.add_0_r (k + context_assumptions Γ)).
-  eapply closedn_ctx_subst; len; simpl.
-  replace (k + context_assumptions Γ + #|Γ|) with (context_assumptions Γ + (k + #|Γ|)) by lia.
-  eapply closedn_ctx_lift => //.
-  eapply forallb_impl. 2:eapply closedn_extended_subst_gen; eauto.
-  simpl; auto.
-Qed.
-
-Lemma closed_ctx_expand_lets Γ Δ : 
-  closed_ctx (Γ ,,, Δ) ->
-  closedn_ctx (context_assumptions Γ) (expand_lets_ctx Γ Δ).
-Proof.
-  rewrite /expand_lets_ctx /expand_lets_k_ctx.
-  intros cl.
-  pose proof (closedn_ctx_subst (context_assumptions Γ) 0).
-  rewrite Nat.add_0_r in H. apply: H.
-  - simpl. len.
-    rewrite closedn_ctx_lift //.
-    rewrite closedn_ctx_app in cl. now move/andP: cl.
-  - apply (closedn_extended_subst_gen Γ 0 0).
-    rewrite closedn_ctx_app in cl.
-    now move/andP: cl => [].
-Qed.
-
-#[global]
-Hint Rewrite to_extended_list_k_length : len.
-
-Lemma smash_context_subst Δ s n Γ : smash_context (subst_context s (n + #|Γ|) Δ) (subst_context s n Γ) =
-  subst_context s n (smash_context Δ Γ).
-Proof.
-  revert Δ. induction Γ as [|[na [b|] ty]]; intros Δ; simpl; auto.
-  - now rewrite Nat.add_0_r.
-  - rewrite -IHΓ.
-    rewrite subst_context_snoc /=. f_equal.
-    rewrite !subst_context_alt !mapi_compose.
-    apply mapi_ext=> n' x.
-    destruct x as [na' [b'|] ty']; simpl.
-    * rewrite !mapi_length /subst_decl /= /map_decl /=; f_equal.
-      + rewrite Nat.add_0_r distr_subst_rec. simpl. lia_f_equal.
-      + rewrite Nat.add_0_r distr_subst_rec; simpl. lia_f_equal.
-    * rewrite !mapi_length /subst_decl /= /map_decl /=; f_equal.
-      rewrite Nat.add_0_r distr_subst_rec /=. lia_f_equal.
-  - rewrite -IHΓ.
-    rewrite subst_context_snoc /= // /subst_decl /map_decl /=.
-    f_equal.
-    rewrite subst_context_app. simpl.
-    rewrite /app_context. f_equal.
-    + lia_f_equal.
-    + rewrite /subst_context // /fold_context_k /= /map_decl /=.
-      lia_f_equal.
-Qed.
-
-
-Lemma smash_context_app_def Γ na b ty :
-  smash_context [] (Γ ++ [{| decl_name := na; decl_body := Some b; decl_type := ty |}]) =
-  smash_context [] (subst_context [b] 0 Γ).
-Proof.
-  now rewrite smash_context_app smash_context_acc /= subst_empty lift0_id lift0_context /=
-    subst_context_nil app_nil_r (smash_context_subst []).
-Qed.
-
-Lemma smash_context_app_ass Γ na ty :
-  smash_context [] (Γ ++ [{| decl_name := na; decl_body := None; decl_type := ty |}]) =
-  smash_context [] Γ ++ [{| decl_name := na; decl_body := None; decl_type := ty |}].
-Proof.
-  rewrite smash_context_app smash_context_acc /= subst_context_lift_id //.
-  now rewrite lift0_context.
-Qed.
-
-Lemma lift_context_add k k' n Γ : lift_context (k + k') n Γ = lift_context k n (lift_context k' n Γ).
-Proof.
-  induction Γ => //.
-  rewrite !lift_context_snoc IHΓ; f_equal.
-  destruct a as [na [b|] ty]; rewrite /lift_decl /map_decl /=; simpl; f_equal;
-  len; rewrite simpl_lift //; try lia.
-Qed.
-
-Lemma distr_lift_subst_context_rec n k s Γ k' : lift_context n (k' + k) (subst_context s k' Γ) =
-  subst_context (map (lift n k) s) k' (lift_context n (#|s| + k + k') Γ).
-Proof.
-  rewrite !lift_context_alt !subst_context_alt.
-  rewrite !mapi_compose.
-  apply mapi_ext.
-  intros n' x.
-  rewrite /lift_decl /subst_decl !compose_map_decl.
-  apply map_decl_ext => y. len.
-  replace (Nat.pred #|Γ| - n' + (#|s| + k + k'))
-    with ((Nat.pred #|Γ| - n' + k') + #|s| + k) by lia.
-  rewrite -distr_lift_subst_rec. f_equal. lia.
-Qed.
-
-Lemma assumption_context_app_inv Γ Δ : assumption_context Γ -> assumption_context Δ ->  
-  assumption_context (Γ ++ Δ).
-Proof.
-  induction 1; try constructor; auto.
-Qed.
-
-Lemma closed_ctx_decl k d Γ : closedn_ctx k (d :: Γ) =
-  closed_decl (k + #|Γ|) d && closedn_ctx k Γ.
-Proof.
-  now simpl; rewrite andb_comm Nat.add_comm.
-Qed.
-
-Lemma closedn_ctx_upwards k k' Γ : 
-  closedn_ctx k Γ -> k <= k' ->
-  closedn_ctx k' Γ.
-Proof.
-  induction Γ; auto. rewrite !closed_ctx_decl /=.
-  move/andb_and => [cla clΓ] le.
-  rewrite (IHΓ clΓ le).
-  rewrite (closed_decl_upwards _ _ cla) //. lia.
-Qed.
-
-Lemma closedn_expand_lets k (Γ : context) t : 
-  closedn (k + context_assumptions Γ) (expand_lets Γ t) -> 
-  closedn (k + #|Γ|) t.
-Proof.
-  revert k t.
-  induction Γ as [|[na [b|] ty] Γ] using ctx_length_rev_ind; intros k t; simpl; auto.
-  - now rewrite /expand_lets /expand_lets_k subst_empty lift0_id.
-  - len.
-    rewrite !expand_lets_vdef.
-    specialize (H (subst_context [b] 0 Γ) ltac:(len; lia)).
-    len in H.
-    intros cl.
-    specialize (H _ _ cl).
-    eapply (closedn_subst_eq' _ k) in H.
-    simpl in *. now rewrite Nat.add_assoc.
-  - len.
-    rewrite !expand_lets_vass. simpl. intros cl.
-    specialize (H Γ ltac:(len; lia)).
-    rewrite (Nat.add_comm _ 1) Nat.add_assoc in cl.
-    now rewrite (Nat.add_comm _ 1) Nat.add_assoc.
-Qed.
-
-
-Ltac len' := rewrite_strat (topdown (repeat (old_hints len))).
-
-Tactic Notation "len'" "in" hyp(id) :=
-  rewrite_strat (topdown (repeat (old_hints len))) in id.
-
-Lemma closedn_expand_lets_eq k (Γ : context) k' t :
-  closedn_ctx k Γ ->
-  closedn (k + k' + context_assumptions Γ) (expand_lets_k Γ k' t) =
-  closedn (k + k' + #|Γ|) t.
-Proof.
-  revert k k' t.
-  induction Γ as [|[na [b|] ty] Γ] using ctx_length_rev_ind; intros k k' t;
-    rewrite ?closedn_ctx_app /= /id /=; simpl; auto.
-  - now rewrite /expand_lets /expand_lets_k /= subst_empty lift0_id.
-  - move/andb_and=> [cld clΓ]. len'.
-    rewrite !expand_lets_k_vdef.
-    simpl in cld |- *. move/andb_and: cld => /= [clb _].
-    specialize (H (subst_context [b] 0 Γ) ltac:(len; lia)).
-    len' in H; simpl in H. len.
-    rewrite H /=.
-    relativize k. eapply closedn_ctx_subst. simpl. 3:rewrite Nat.add_0_r //.
-    now rewrite Nat.add_0_r. now rewrite /= clb.
-    rewrite -Nat.add_assoc -closedn_subst_eq. simpl. now rewrite clb.
-    simpl; lia_f_equal.
-  - len'. move/andb_and => [clty clΓ]. 
-    rewrite !expand_lets_k_vass. simpl.
-    specialize (H Γ ltac:(len; lia) (S k)).
-    rewrite Nat.add_assoc !Nat.add_succ_r !Nat.add_0_r. apply H.
-    now rewrite Nat.add_1_r in clΓ.
-Qed.
-
-Lemma closedn_to_extended_list_k_up k Γ k' : 
-  k' + #|Γ| <= k ->
-  forallb (closedn k) (to_extended_list_k Γ k').
-Proof.
-  move=> le. rewrite /to_extended_list_k.
-  eapply Forall_forallb; eauto. 2:{ intros x H; eapply H. }
-  eapply Forall_impl. eapply reln_list_lift_above. constructor.
-  simpl; intros.
-  destruct H as [n [-> leq]]. simpl.
-  eapply Nat.ltb_lt. lia.
-Qed.
-
-Lemma closedn_to_extended_list_k Γ k : 
-  forallb (closedn (k + #|Γ|)) (to_extended_list_k Γ k).
-Proof.
-  now apply closedn_to_extended_list_k_up.
-Qed.
-
-Lemma closedn_to_extended_list Γ : 
-  forallb (closedn #|Γ|) (to_extended_list Γ).
-Proof.
-  rewrite /to_extended_list.
-  apply (closedn_to_extended_list_k _ 0).
-Qed.
-
-Lemma closed_ind_predicate_context {Σ ind mdecl idecl} : 
-  declared_inductive Σ ind mdecl idecl ->
-  closed_inductive_decl mdecl ->
-  closedn_ctx (context_assumptions mdecl.(ind_params)) (ind_predicate_context ind mdecl idecl).
-Proof.
-  intros decli cl.
-  move: (closed_declared_ind decli cl).
-  move/andP: cl => [] clpars _.
-  move/andP => [] /andP [] /andP [] clty clinds _ _.
-  rewrite /ind_predicate_context /=.
-  apply/andP. split.
-  - now eapply (closedn_ctx_expand_lets 0).
-  - rewrite /test_decl /=; len.
-    rewrite closedn_mkApps /= //.
-    set foo := (X in forallb X _).
-    relativize foo.
-    eapply closedn_to_extended_list.
-    now rewrite /foo; len.
-Qed.
-
-Lemma closed_inds {ind mdecl u} :
-  forallb (closedn 0) (inds (inductive_mind ind) u (ind_bodies mdecl)).
-Proof.
-  rewrite inds_spec. rewrite forallb_rev.
-  unfold mapi.
-  generalize 0 at 2.
-  induction (ind_bodies mdecl); simpl; auto.
-Qed.
 
 Lemma declared_minductive_closed_inds {cf:checker_flags} {Σ ind mdecl u} {wfΣ : wf Σ} :
   declared_minductive Σ (inductive_mind ind) mdecl ->
@@ -1162,6 +313,7 @@ Proof.
   - simpl. eauto.
 Qed.
 
+
 Lemma closed_cstr_branch_context_gen {cf : checker_flags} {Σ} {wfΣ : wf Σ} {c mdecl cdecl} : 
   closed_inductive_decl mdecl ->
   closed_constructor_body mdecl cdecl ->
@@ -1172,21 +324,10 @@ Proof.
   move/andP: clc => [] /andP [] clargs clinds cltype.
   rewrite /cstr_branch_context /=.
   eapply (closedn_ctx_expand_lets 0) => // /=.
-  eapply closedn_ctx_subst. len. now rewrite Nat.add_comm.
+  eapply (closedn_ctx_subst 0). len. now rewrite Nat.add_comm.
   eapply closed_inds.
 Qed.
 
-Lemma closed_ind_closed_cstrs {Σ ind mdecl idecl} : 
-  closed_inductive_decl mdecl -> 
-  declared_inductive Σ ind mdecl idecl ->
-  All (closed_constructor_body mdecl) (ind_ctors idecl).
-Proof.
-  intros []%andb_and.
-  intros [decli hnth].
-  solve_all. eapply nth_error_all in H0; tea.
-  simpl in H0.
-  move/andP: H0 => [] /andP []; solve_all.
-Qed.
 
 Lemma typecheck_closed `{cf : checker_flags} :
   env_prop (fun Σ Γ t T =>
@@ -1198,7 +339,7 @@ Proof.
   rewrite -> ?andb_and in *; try solve [intuition auto].
 
   - induction X0; auto; rewrite closedn_ctx_cons /= IHX0 /= //.
-    now move/andP: p => [] /= -> _.
+    now move/andP: p => [] /=. 
 
   - pose proof (nth_error_Some_length H).
     elim (Nat.ltb_spec n #|Γ|); intuition auto. all: try lia. clear H1.
@@ -1282,8 +423,9 @@ Proof.
         rewrite (wf_predicate_length_pars H1).
         now rewrite (declared_minductive_ind_npars isdecl).
       * rewrite (All2_length a1).
-        len in H8.
-        rewrite case_branch_type_fst in H8.
+        len in H8. 
+        (*unfold case_branch_context_gen in H8. simpl in H8.
+        rewrite case_branch_type_fst in H8. *)
         rewrite case_branch_context_length_args in H8 => //.
         now rewrite cstr_branch_context_length.
     + rewrite closedn_mkApps; auto.
@@ -1344,6 +486,7 @@ Proof.
   solve_all. eapply nth_error_all in cli; eauto.
   now simpl in cli.
 Qed.
+ 
 
 Lemma declared_projection_closed {cf:checker_flags} {Σ : global_env} {wfΣ : wf Σ}{mdecl idecl p cdecl pdecl} : 
   declared_projection Σ p mdecl idecl cdecl pdecl ->
@@ -1385,7 +528,32 @@ Proof.
   eapply nth_error_all in clc; eauto. now simpl in clc.
 Qed.
 
+
 Implicit Types (cf : checker_flags) (Σ : global_env_ext).
+
+Lemma closedn_All_local_closed:
+  forall (cf : checker_flags) (Σ : global_env_ext) (Γ : context) (ctx : list context_decl)
+         (wfΓ' : wf_local Σ (Γ ,,, ctx)),
+    All_local_env_over typing
+    (fun (Σ0 : global_env_ext) (Γ0 : context) (_ : wf_local Σ0 Γ0) (t T : term) (_ : Σ0;;; Γ0 |- t : T) =>
+       closedn #|Γ0| t && closedn #|Γ0| T) Σ (Γ ,,, ctx) wfΓ' ->
+    closedn_ctx 0 Γ && closedn_ctx #|Γ| ctx.
+Proof.
+  intros cf Σ Γ ctx wfΓ' al.
+  remember (Γ ,,, ctx) as Γ'. revert Γ' wfΓ' ctx HeqΓ' al.
+  induction Γ. simpl. intros. subst. unfold app_context in *. rewrite app_nil_r in wfΓ' al.
+  induction al; try constructor;
+  rewrite closedn_ctx_cons /=; cbn.
+  move/andP: p => [] /= -> _. now rewrite IHal.
+  now rewrite IHal /= /test_decl /=.
+  intros.
+  unfold app_context in *. subst Γ'.
+  specialize (IHΓ (ctx ++ a :: Γ) wfΓ' (ctx ++ [a])).
+  rewrite -app_assoc in IHΓ. specialize (IHΓ eq_refl al).
+  rewrite closedn_ctx_app /= Nat.add_1_r andb_assoc in IHΓ.
+  now rewrite closedn_ctx_cons /=.
+Qed.
+
 
 Lemma subject_closed {cf} {Σ} {wfΣ : wf Σ.1} {Γ t T} : 
   Σ ;;; Γ |- t : T ->
@@ -1621,6 +789,135 @@ Proof.
   now eapply declared_projection_closed in decl.
 Qed.
   
+
+Hint Unfold inst_case_branch_context : len.
+
+(** This shows preservation by reduction of closed/noccur_between predicates 
+  necessary to prove exchange and strengthening lemmas. *)
+Lemma red1_on_free_vars {cf:checker_flags} {P : nat -> bool} {Σ Γ u v} {wfΣ : wf Σ} :
+  red1 Σ Γ u v ->
+  on_free_vars P u ->
+  on_ctx_free_vars P Γ ->
+  on_free_vars P v.
+Proof.
+  intros h hav hctx.
+  induction h using red1_ind_all in P, hav, hctx |- *.
+  all: try solve [
+    simpl ; constructor ; eapply IHh ;
+    try (simpl in hav; rtoProp);
+    try eapply urenaming_vass ;
+    try eapply urenaming_vdef ;
+    assumption
+  ].
+  all:simpl in hav |- *; try toAll.
+  all:try move/and3P: hav => [h1 h2 h3].
+  all:try (move/andP: hav => [] /andP [] h1 h2 h3).
+  all:try move/andP: hav => [h1 h2].
+  all:try move/andP: h3 => [] h3 h4.
+  all:try move/andP: h4 => [] h4 h5.
+  all:try rewrite ?h1 // ?h2 // ?h3 // ?h4 // ?IHh /= // ?andb_true_r.
+  all:try eapply on_free_vars_subst1; eauto.
+  - destruct (nth_error Γ i) eqn:hnth => //.
+    simpl in H. noconf H.
+    epose proof (nth_error_on_free_vars_ctx P 0 Γ i c).
+    forward H0. { now rewrite addnP0. }
+    specialize (H0 hav hnth). simpl in H0.
+    rewrite /test_decl H in H0.
+    rewrite on_free_vars_lift0 //.
+    now move/andP: H0 => [] /=.
+  - rewrite /iota_red.
+    rename h5 into hbrs.
+    move: h4. rewrite on_free_vars_mkApps => /andP [] /= _ hargs.
+    apply on_free_vars_subst.
+    { rewrite forallb_rev forallb_skipn //. }
+    len.
+    rewrite H0.
+    rewrite /expand_lets /expand_lets_k /=.
+    eapply forallb_nth_error in hbrs.
+    erewrite H in hbrs; simpl in hbrs.
+    move/andP: hbrs => [] hbr hbody.
+    eapply on_free_vars_subst.
+    * relativize (context_assumptions _).
+      + unshelve eapply foron_free_vars_extended_subst. eauto.
+        eapply on_free_vars_ctx_inst_case_context; tea => //.
+      + unfold inst_case_branch_context. now len. 
+    * rewrite extended_subst_length.
+      rewrite shiftnP_add.
+      eapply on_free_vars_lift_impl in hbody. unfold inst_case_branch_context. len.
+      now rewrite Nat.add_comm.
+  - rewrite !on_free_vars_mkApps in hav |- *.
+    rtoProp.
+    eapply on_free_vars_unfold_fix in H; eauto. 
+  - move: h4; rewrite !on_free_vars_mkApps.
+    move=> /andP [] hcofix ->.
+    eapply on_free_vars_unfold_cofix in hcofix; eauto.
+    now rewrite hcofix.
+  - move: hav; rewrite !on_free_vars_mkApps => /andP [] hcofix ->.
+    eapply on_free_vars_unfold_cofix in H as ->; eauto.
+  - eapply closed_on_free_vars. rewrite closedn_subst_instance.
+    eapply declared_constant_closed_body; eauto.
+  - move: hav; rewrite on_free_vars_mkApps /=.
+    now move/(nth_error_forallb H).
+  - rewrite (on_ctx_free_vars_concat _ _ [_]) // /= hctx
+      on_ctx_free_vars_tip /= addnP_shiftnP /on_free_vars_decl
+      /test_decl /= // hctx h2.
+  - rewrite (on_ctx_free_vars_concat _ _ [_]) // hctx
+      on_ctx_free_vars_tip /= addnP_shiftnP /on_free_vars_decl /test_decl /= h2 /=
+      /foroptb /= h1 // h2.
+  - solve_all.
+    + eapply OnOne2_impl_All_r; eauto. solve_all.
+    + now rewrite -(OnOne2_length X).
+    + now rewrite -(OnOne2_length X).
+  - relativize #|pcontext p|; unfold inst_case_predicate_context.
+    * erewrite on_ctx_free_vars_extend; rewrite // hctx.
+      erewrite on_free_vars_ctx_inst_case_context => //.
+    * now len.
+  - toAll.
+    clear -h1 hctx X h5.
+    eapply OnOne2_All_mix_left in X; tea.
+    toAll. eapply OnOne2_impl_All_r in X; tea; solve_all; rewrite -?b0 //.
+    eapply b1 => //.
+    relativize #|bcontext x|; unfold inst_case_branch_context.
+    * erewrite on_ctx_free_vars_extend; rewrite // hctx.
+      erewrite on_free_vars_ctx_inst_case_context => //. solve_all.
+    * now len.
+  - rewrite (on_ctx_free_vars_concat _ _ [_]) // /= hctx
+      on_ctx_free_vars_tip /= addnP_shiftnP /on_free_vars_decl /test_decl /= h1 /= //.
+  - toAll. eapply OnOne2_impl_All_r; eauto; solve_all.
+  - toAll. unfold test_def.
+    rewrite -(OnOne2_length X).
+    eapply OnOne2_impl_All_r; eauto; solve_all.
+    destruct x, y; noconf b; simpl in *. rtoProp; solve_all.
+  - toAll. unfold test_def in *. rewrite -(OnOne2_length X).
+    eapply OnOne2_impl_All_r; eauto; solve_all;
+     destruct x, y; noconf b; simpl in *; rtoProp; solve_all.
+    apply b0 => //.
+    rewrite -(fix_context_length mfix0).
+    erewrite on_ctx_free_vars_extend; rewrite // hctx.
+    now apply on_free_vars_fix_context.
+  - toAll. unfold test_def.
+    rewrite -(OnOne2_length X).
+    eapply OnOne2_impl_All_r; eauto; solve_all.
+    destruct x, y; noconf b; simpl in *. rtoProp; solve_all.
+  - toAll. unfold test_def in *. rewrite -(OnOne2_length X).
+    eapply OnOne2_impl_All_r; eauto; solve_all;
+    destruct x, y; noconf b; simpl in *; rtoProp; solve_all.
+    apply b0 => //.
+    rewrite -(fix_context_length mfix0).
+    rewrite on_ctx_free_vars_extend // hctx.
+    now apply on_free_vars_fix_context.
+Qed.
+
+Lemma red_on_free_vars {cf} {P : nat -> bool} {Σ Γ u v} {wfΣ : wf Σ} :
+  red Σ Γ u v ->
+  on_free_vars P u ->
+  on_ctx_free_vars P Γ ->
+  on_free_vars P v.
+Proof.
+  induction 1; eauto using red1_on_free_vars.
+Qed.
+
+
 Lemma term_closedn_list_ind :
   forall (P : nat -> term -> Type), 
     (forall k (n : nat), n < k -> P k (tRel n)) ->
