pcuic/theories/PCUICCumulativitySpec.v
@@ -1,171 +1,241 @@
 (* Distributed under the terms of the MIT license. *)
 From Coq Require Import CRelationClasses.
 From Equations.Type Require Import Relation Relation_Properties.
-From MetaCoq.Template Require Import config utils BasicAst.
+From MetaCoq.Template Require Import config utils BasicAst Reflect.
 From MetaCoq.PCUIC Require Import PCUICAst PCUICAstUtils PCUICEquality
-     PCUICLiftSubst PCUICUnivSubst PCUICContextRelation PCUICCases.
+     PCUICLiftSubst PCUICUnivSubst PCUICContextRelation PCUICCases PCUICOnFreeVars.
 
 Set Default Goal Selector "!".
 
-(** * Definition of cumulativity and conversion relations *)
-
-
-(* todo mode typing notation *)
 Reserved Notation " Σ ;;; Γ |- t <=s u " (at level 50, Γ, t, u at next level).
 Reserved Notation " Σ ;;; Γ |- t =s u " (at level 50, Γ, t, u at next level).
 
-(** ** Cumulativity *)
+(** * Definition of cumulativity and conversion relations *)
 
-Inductive cumulSpec (Σ : global_env) (Re Rle : Universe.t -> Universe.t -> Prop) (Γ : context) : term -> term -> Type :=
+Inductive cumulSpec0 (Σ : global_env) (Re Rle : Universe.t -> Universe.t -> Prop) (Γ : context) : term -> term -> Type :=
 
 (* transitivity *)
 
 | cumul_Trans t u v :
-    cumulSpec Σ Re Rle Γ t u ->
-    cumulSpec Σ Re Rle Γ u v ->    
-    cumulSpec Σ Re Rle Γ t v 
+    is_closed_context Γ -> is_open_term Γ u -> 
+    cumulSpec0 Σ Re Rle Γ t u ->
+    cumulSpec0 Σ Re Rle Γ u v ->    
+    cumulSpec0 Σ Re Rle Γ t v 
 
 (* symmetry *)
 
 | cumul_Sym t u :
-    cumulSpec Σ Re Rle Γ t u ->
-    cumulSpec Σ Re Rle Γ u t  
+    cumulSpec0 Σ Re Re Γ t u ->
+    cumulSpec0 Σ Re Rle Γ u t  
 
 (* reflexivity *)
 
 | cumul_Refl t :
-    cumulSpec Σ Re Rle Γ t t 
+    cumulSpec0 Σ Re Rle Γ t t 
 
 (* Cumulativity rules *)
 
 | cumul_Ind i u u' args args':
     R_global_instance Σ Re Rle (IndRef i) #|args| u u' ->
-    #|args| = #|args'| ->
-    All2 (cumulSpec Σ Re Re Γ) args args' ->
-    cumulSpec Σ Re Rle Γ (mkApps (tInd i u) args) (mkApps (tInd i u') args')
+    All2 (cumulSpec0 Σ Re Re Γ) args args' ->
+    cumulSpec0 Σ Re Rle Γ (mkApps (tInd i u) args) (mkApps (tInd i u') args')
 
 | cumul_Construct i k u u' args args':
     R_global_instance Σ Re Rle (ConstructRef i k) #|args| u u' ->
-    #|args| = #|args'| ->
-    All2 (cumulSpec Σ Re Re Γ) args args' ->
-    cumulSpec Σ Re Rle Γ (mkApps (tConstruct i k u) args) (mkApps (tConstruct i k u') args')
+    All2 (cumulSpec0 Σ Re Re Γ) args args' ->
+    cumulSpec0 Σ Re Rle Γ (mkApps (tConstruct i k u) args) (mkApps (tConstruct i k u') args')
 
 | cumul_Sort s s' :
     Rle s s' ->
-    cumulSpec Σ Re Rle Γ (tSort s) (tSort s')
+    cumulSpec0 Σ Re Rle Γ (tSort s) (tSort s')
 
 | cumul_Const c u u' :
     R_universe_instance Re u u' ->
-    cumulSpec Σ Re Rle Γ (tConst c u) (tConst c u')
+    cumulSpec0 Σ Re Rle Γ (tConst c u) (tConst c u')
 
 (* congruence rules *)
 
 | cumul_Evar e args args' :
-    All2 (cumulSpec Σ Re Re Γ) args args' ->
-    cumulSpec Σ Re Rle Γ (tEvar e args) (tEvar e args')
+    All2 (cumulSpec0 Σ Re Re Γ) args args' ->
+    cumulSpec0 Σ Re Rle Γ (tEvar e args) (tEvar e args')
 
 | cumul_App t t' u u' :
-    cumulSpec Σ Re Rle Γ t t' ->
-    cumulSpec Σ Re Re Γ u u' ->
-    cumulSpec Σ Re Rle Γ (tApp t u) (tApp t' u')
+    cumulSpec0 Σ Re Rle Γ t t' ->
+    cumulSpec0 Σ Re Re Γ u u' ->
+    cumulSpec0 Σ Re Rle Γ (tApp t u) (tApp t' u')
 
 | cumul_Lambda na na' ty ty' t t' :
     eq_binder_annot na na' ->
-    cumulSpec Σ Re Re Γ ty ty' ->
-    cumulSpec Σ Re Rle Γ t t' ->
-    cumulSpec Σ Re Rle Γ (tLambda na ty t) (tLambda na' ty' t')
+    cumulSpec0 Σ Re Re Γ ty ty' ->
+    cumulSpec0 Σ Re Rle Γ t t' ->
+    cumulSpec0 Σ Re Rle Γ (tLambda na ty t) (tLambda na' ty' t')
 
 | cumul_Prod na na' a a' b b' :
     eq_binder_annot na na' ->
-    cumulSpec Σ Re Re Γ a a' ->
-    cumulSpec Σ Re Rle Γ b b' ->
-    cumulSpec Σ Re Rle Γ (tProd na a b) (tProd na' a' b')
+    cumulSpec0 Σ Re Re Γ a a' ->
+    cumulSpec0 Σ Re Rle Γ b b' ->
+    cumulSpec0 Σ Re Rle Γ (tProd na a b) (tProd na' a' b')
 
 | cumul_LetIn na na' t t' ty ty' u u' :
     eq_binder_annot na na' ->
-    cumulSpec Σ Re Re Γ t t' ->
-    cumulSpec Σ Re Re Γ ty ty' ->
-    cumulSpec Σ Re Rle Γ u u' ->
-    cumulSpec Σ Re Rle Γ (tLetIn na t ty u) (tLetIn na' t' ty' u')
+    cumulSpec0 Σ Re Re Γ t t' ->
+    cumulSpec0 Σ Re Re Γ ty ty' ->
+    cumulSpec0 Σ Re Rle Γ u u' ->
+    cumulSpec0 Σ Re Rle Γ (tLetIn na t ty u) (tLetIn na' t' ty' u')
 
 | cumul_Case indn p p' c c' brs brs' :
-    eq_predicate (cumulSpec Σ Re Re Γ) Re p p' ->
-    cumulSpec Σ Re Re Γ c c' ->
+    eq_predicate (cumulSpec0 Σ Re Re Γ) Re p p' ->
+    cumulSpec0 Σ Re Re Γ c c' ->
     All2 (fun x y =>
       eq_context_gen eq eq (bcontext x) (bcontext y) *
-      cumulSpec Σ Re Re Γ (bbody x) (bbody y)
+      cumulSpec0 Σ Re Re Γ (bbody x) (bbody y)
     ) brs brs' ->
-    cumulSpec Σ Re Rle Γ (tCase indn p c brs) (tCase indn p' c' brs')
+    cumulSpec0 Σ Re Rle Γ (tCase indn p c brs) (tCase indn p' c' brs')
 
 | cumul_Proj p c c' :
-    cumulSpec Σ Re Re Γ c c' ->
-    cumulSpec Σ Re Rle Γ (tProj p c) (tProj p c')
+    cumulSpec0 Σ Re Re Γ c c' ->
+    cumulSpec0 Σ Re Rle Γ (tProj p c) (tProj p c')
 
 | cumul_Fix mfix mfix' idx :
     All2 (fun x y =>
-      cumulSpec Σ Re Re Γ x.(dtype) y.(dtype) *
-      cumulSpec Σ Re Re Γ x.(dbody) y.(dbody) *
+      cumulSpec0 Σ Re Re Γ x.(dtype) y.(dtype) *
+      cumulSpec0 Σ Re Re Γ x.(dbody) y.(dbody) *
       (x.(rarg) = y.(rarg)) *
       eq_binder_annot x.(dname) y.(dname)
     )%type mfix mfix' ->
-    cumulSpec Σ Re Rle Γ (tFix mfix idx) (tFix mfix' idx)
+    cumulSpec0 Σ Re Rle Γ (tFix mfix idx) (tFix mfix' idx)
 
 | cumul_CoFix mfix mfix' idx :
     All2 (fun x y =>
-      cumulSpec Σ Re Re Γ x.(dtype) y.(dtype) *
-      cumulSpec Σ Re Re Γ x .(dbody) y.(dbody) *
+      cumulSpec0 Σ Re Re Γ x.(dtype) y.(dtype) *
+      cumulSpec0 Σ Re Re Γ x .(dbody) y.(dbody) *
       (x.(rarg) = y.(rarg)) *
       eq_binder_annot x.(dname) y.(dname)
     ) mfix mfix' ->
-    cumulSpec Σ Re Rle Γ (tCoFix mfix idx) (tCoFix mfix' idx)
+    cumulSpec0 Σ Re Rle Γ (tCoFix mfix idx) (tCoFix mfix' idx)
 
 (** Reductions *)
 
 (** Beta red *)
 | cumul_beta na t b a :
-    cumulSpec Σ Re Rle Γ (tApp (tLambda na t b) a) (subst10 a b)
+    cumulSpec0 Σ Re Rle Γ (tApp (tLambda na t b) a) (subst10 a b)
 
 (** Let *)
 | cumul_zeta na b t b' :
-    cumulSpec Σ Re Rle Γ (tLetIn na b t b') (subst10 b b')
+    cumulSpec0 Σ Re Rle Γ (tLetIn na b t b') (subst10 b b')
 
 | cumul_rel i body :
     option_map decl_body (nth_error Γ i) = Some (Some body) ->
-    cumulSpec Σ Re Rle Γ (tRel i) (lift0 (S i) body)
+    cumulSpec0 Σ Re Rle Γ (tRel i) (lift0 (S i) body)
 
 (** iota red *)
 | cumul_iota ci c u args p brs br :
     nth_error brs c = Some br ->
     #|skipn (ci_npar ci) args| = context_assumptions br.(bcontext) ->
-    cumulSpec Σ Re Rle Γ (tCase ci p (mkApps (tConstruct ci.(ci_ind) c u) args) brs)
+    cumulSpec0 Σ Re Rle Γ (tCase ci p (mkApps (tConstruct ci.(ci_ind) c u) args) brs)
                          (iota_red ci.(ci_npar) p args br)
 
 (** Fix unfolding, with guard *)
 | cumul_fix mfix idx args narg fn :
     unfold_fix mfix idx = Some (narg, fn) ->
     is_constructor narg args = true ->
-    cumulSpec Σ Re Rle Γ (mkApps (tFix mfix idx) args)
+    cumulSpec0 Σ Re Rle Γ (mkApps (tFix mfix idx) args)
                          (mkApps fn args)
 
 (** CoFix-case unfolding *)
 | cumul_cofix_case ip p mfix idx args narg fn brs :
     unfold_cofix mfix idx = Some (narg, fn) ->
-    cumulSpec Σ Re Rle Γ (tCase ip p (mkApps (tCoFix mfix idx) args) brs)
+    cumulSpec0 Σ Re Rle Γ (tCase ip p (mkApps (tCoFix mfix idx) args) brs)
                          (tCase ip p (mkApps fn args) brs)
 
 (** CoFix-proj unfolding *)
 | cumul_cofix_proj p mfix idx args narg fn :
     unfold_cofix mfix idx = Some (narg, fn) ->
-    cumulSpec Σ Re Rle Γ (tProj p (mkApps (tCoFix mfix idx) args))
+    cumulSpec0 Σ Re Rle Γ (tProj p (mkApps (tCoFix mfix idx) args))
                          (tProj p (mkApps fn args))
 
 (** Constant unfolding *)
 | cumul_delta c decl body (isdecl : declared_constant Σ c decl) u :
     decl.(cst_body) = Some body ->
-    cumulSpec Σ Re Rle Γ (tConst c u) (subst_instance u body)
+    cumulSpec0 Σ Re Rle Γ (tConst c u) (subst_instance u body)
 
 (** Proj *)
 | cumul_proj i pars narg args u arg:
     nth_error args (pars + narg) = Some arg ->
-    cumulSpec Σ Re Rle Γ (tProj (i, pars, narg) (mkApps (tConstruct i 0 u) args)) arg.
+    cumulSpec0 Σ Re Rle Γ (tProj (i, pars, narg) (mkApps (tConstruct i 0 u) args)) arg.
 
+Definition convSpec `{checker_flags} Σ :=
+  let φ := (global_ext_constraints Σ) in cumulSpec0 Σ.1 (eq_universe φ) (eq_universe φ).
+
+(* ** Syntactic cumulativity up-to universes *)
+
+Definition cumulSpec `{checker_flags} Σ :=
+  let φ := (global_ext_constraints Σ) in cumulSpec0 Σ.1 (eq_universe φ) (leq_universe φ).
+
+Notation " Σ ;;; Γ |- t <=s u " := (@cumulSpec _ Σ Γ t u).
+Notation " Σ ;;; Γ |- t =s u " := (@convSpec _ Σ Γ t u).
+  
+Module PCUICConversionParSpec <: EnvironmentTyping.ConversionParSig PCUICTerm PCUICEnvironment PCUICEnvTyping.
+  Definition conv := @convSpec.
+  Definition cumul := @cumulSpec.
+End PCUICConversionParSpec.
+
+Module PCUICConversionSpec := EnvironmentTyping.Conversion PCUICTerm PCUICEnvironment PCUICEnvTyping PCUICConversionParSpec.
+Include PCUICConversionSpec.
+
+Notation conv_context Σ Γ Γ' := (All2_fold (conv_decls Σ) Γ Γ').
+Notation cumul_context Σ Γ Γ' := (All2_fold (cumul_decls Σ) Γ Γ').
+
+
+#[global]
+Instance conv_decls_refl {cf:checker_flags} Σ Γ Γ' : Reflexive (conv_decls Σ Γ Γ').
+Proof.
+  intros x. destruct x as [na [b|] ty]; constructor; auto.
+  all:constructor; apply eq_term_refl.
+Qed.
+
+#[global]
+Instance cumul_decls_refl {cf:checker_flags} Σ Γ Γ' : Reflexive (cumul_decls Σ Γ Γ').
+Proof.
+  intros x. destruct x as [na [b|] ty]; constructor; auto.
+  all:constructor; apply eq_term_refl || apply leq_term_refl.
+Qed.
+
+#[global]
+Instance cumul_refl' {cf:checker_flags} Σ Γ : Reflexive (cumulSpec Σ Γ).
+Proof.
+  intro. constructor 3.
+Qed.
+
+#[global]
+Instance conv_refl' {cf:checker_flags} Σ Γ : Reflexive (convSpec Σ Γ).
+Proof.
+  intro; constructor 3. 
+Qed.
+
+Section ContextConversion.
+  Context {cf : checker_flags}.
+  Context (Σ : global_env_ext).
+
+  Notation conv_context Γ Γ' := (All2_fold (conv_decls Σ) Γ Γ').
+  Notation cumul_context Γ Γ' := (All2_fold (cumul_decls Σ) Γ Γ').
+
+  Global Instance conv_ctx_refl : Reflexive (All2_fold (conv_decls Σ)).
+  Proof.
+    intro Γ; induction Γ; try econstructor; auto.
+    reflexivity.
+  Qed.
+
+  Global Instance cumul_ctx_refl : Reflexive (All2_fold (cumul_decls Σ)).
+  Proof.
+    intro Γ; induction Γ; try econstructor; auto.
+    reflexivity. 
+  Qed.
+
+  Definition conv_ctx_refl' Γ : conv_context Γ Γ
+  := conv_ctx_refl Γ.
+
+  Definition cumul_ctx_refl' Γ : cumul_context Γ Γ
+    := cumul_ctx_refl Γ.
+
+End ContextConversion.
