pcuic/theories/Conversion/PCUICNamelessConv.v
@@ -1,10 +1,10 @@
 (* Distributed under the terms of the MIT license. *)
 From Coq Require Import RelationClasses.
 From MetaCoq.Template Require Import config utils.
-From MetaCoq.PCUIC Require Import PCUICAst PCUICAstUtils PCUICInduction
-     PCUICLiftSubst PCUICEquality PCUICTyping PCUICPosition PCUICUnivSubst
-     PCUICContextRelation PCUICNamelessDef PCUICGuardCondition
-     PCUICSigmaCalculus (* for context manipulations *).
+From MetaCoq.PCUIC Require Import PCUICAst PCUICAstUtils PCUICInduction PCUICCases
+     PCUICLiftSubst PCUICEquality PCUICReduction PCUICCumulativitySpec PCUICCumulativity PCUICPosition PCUICUnivSubst
+     PCUICContextRelation PCUICNamelessDef PCUICGuardCondition PCUICClosedTyping PCUICUnivSubstitutionConv
+     PCUICClosed PCUICSigmaCalculus (* for context manipulations *).
 Require Import Equations.Prop.DepElim.
 Require Import ssreflect.
 
@@ -653,26 +653,6 @@ Proof.
   rewrite h. reflexivity.
 Qed.
 
-Lemma nlg_wf_local {cf : checker_flags} :
-  forall Σ Γ (hΓ : wf_local Σ Γ),
-    All_local_env_over
-      typing
-      (fun Σ Γ (_ : wf_local Σ Γ) (t T : term) (_ : Σ ;;; Γ |- t : T) =>
-         nlg Σ ;;; nlctx Γ |- nl t : nl T)
-      Σ Γ hΓ ->
-    wf_local (nlg Σ) (nlctx Γ).
-Proof.
-  intros Σ Γ hΓ h.
-  induction h.
-  - constructor.
-  - simpl. unfold map_decl_anon. cbn. constructor. 1: assumption.
-    eexists. exact p.
-  - simpl. unfold map_decl_anon. cbn. constructor.
-    + assumption.
-    + eexists. exact p0.
-    + assumption.
-Qed.
-
 Lemma All_mapi_spec {A B} {P : A -> Type} {l} {f g : nat -> A -> B} {n} :
   All P l -> (forall n x, P x -> f n x = g n x) ->
   mapi_rec f l n = mapi_rec g l n.
@@ -874,7 +854,6 @@ Proof.
     + unfold map_decl_anon. cbn. rewrite nl_lift. reflexivity.
 Qed.
 
-From MetaCoq.PCUIC Require Import PCUICCases.
 
 Lemma nl_declared_inductive Σ ind mdecl idecl :
   declared_inductive Σ ind mdecl idecl ->
@@ -898,7 +877,6 @@ Proof.
   - now eapply nl_declared_inductive.
   - simpl. now rewrite nth_error_map H0.
 Qed.
-From MetaCoq.PCUIC Require Import PCUICUnivSubstitution.
 
 Lemma nl_to_extended_list:
   forall indctx : list context_decl,
@@ -1243,8 +1221,6 @@ Proof.
   apply nl_wf_branch.
 Qed.
 
-From MetaCoq.PCUIC Require Import PCUICClosed.
-
 Lemma closed_ctx_IH :
   forall (l : list context_decl) (n : nat),
   onctx_k (fun (k : nat) (t : term) => closedn k (nl t)) n l ->
@@ -1469,58 +1445,6 @@ Proof.
 Qed.
 #[global] Hint Resolve nl_cumul_ctx : nl.
 
-Lemma nl_check_one_fix d : check_one_fix d = check_one_fix (map_def_anon nl nl d).
-Proof.
-  destruct d; simpl.
-  rewrite (nl_decompose_prod_assum [] dtype).
-  destruct decompose_prod_assum.
-  rewrite -(nlctx_smash_context []) -map_rev nth_error_map.
-  destruct nth_error => //. cbn.
-  rewrite [decompose_app_rec _ _]nl_decompose_app.
-  destruct decompose_app => //.
-  destruct t0 => //.
-Qed.
-
-Lemma nl_wf_fixpoint Σ mfix :
-  wf_fixpoint Σ.1 mfix = wf_fixpoint (nlg Σ).1 (map (map_def_anon nl nl) mfix).
-Proof.
-  unfold wf_fixpoint.
-  replace (map check_one_fix mfix) with (map check_one_fix (map (map_def_anon nl nl) mfix)) => //.
-  * destruct map_option_out => //. destruct l => //.
-    f_equal. rewrite /check_recursivity_kind.
-    epose proof (nl_lookup_env Σ.1).
-    destruct Σ; cbn in *. rewrite H.
-    destruct lookup_env => //. cbn.
-    destruct g0 => //.
-  * rewrite map_map_compose.
-    now setoid_rewrite <-nl_check_one_fix.
-Qed.
-
-Lemma nl_check_one_cofix d : check_one_cofix d = check_one_cofix (map_def_anon nl nl d).
-Proof.
-  destruct d; simpl.
-  rewrite (nl_decompose_prod_assum [] dtype).
-  destruct decompose_prod_assum.
-  rewrite nl_decompose_app.
-  destruct decompose_app => //.
-  destruct t0 => //.
-Qed.
-
-Lemma nl_wf_cofixpoint Σ mfix :
-  wf_cofixpoint Σ.1 mfix = wf_cofixpoint (nlg Σ).1 (map (map_def_anon nl nl) mfix).
-Proof.
-  unfold wf_cofixpoint.  
-  replace (map check_one_cofix mfix) with (map check_one_cofix (map (map_def_anon nl nl) mfix)) => //.
-  * destruct map_option_out => //. destruct l => //.
-    f_equal. rewrite /check_recursivity_kind.
-    epose proof (nl_lookup_env Σ.1).
-    destruct Σ; cbn in *. rewrite H.
-    destruct lookup_env => //. cbn.
-    destruct g0 => //.
-  * rewrite map_map_compose.
-    now setoid_rewrite <- nl_check_one_cofix.
-Qed.
-
 Lemma nl_monomorphic_levels_decl g : monomorphic_levels_decl (nl_global_decl g) = monomorphic_levels_decl g.
 Proof.
   destruct g; simpl.
@@ -1542,12 +1466,6 @@ Proof.
   intros x. now rewrite !LevelSet.union_spec nl_global_levels.
 Qed.
 
-Lemma wf_universe_nl Σ u : wf_universe Σ u -> wf_universe (nlg Σ) u.
-Proof.
-  destruct u; simpl; auto.
-  intros.
-  now rewrite nl_global_ext_levels.
-Qed.
 
 Lemma All2i_map {A B C D} (f : A -> B) (g : C -> D) P n l l' : 
   All2i (fun i x y => P i (f x) (g y)) n l l' <~>
@@ -1565,164 +1483,6 @@ Proof.
   now rewrite global_ext_constraints_nlg.
 Qed.
 
-Lemma typing_nlg {cf : checker_flags} :
-  env_prop (fun Σ Γ t T => nlg Σ ;;; nlctx Γ |- nl t : nl T)
-    (fun Σ Γ => wf_local (nlg Σ) (nlctx Γ)).
-Proof.
-  clear.
-  apply typing_ind_env; intros; cbn in *;
-    rewrite ?nl_lift ?nl_subst ?nl_subst_instance;
-    try (econstructor; eauto using nlg_wf_local; fail).
-  - induction X; simpl; constructor; auto.
-    * now exists (tu.π1).
-    * now exists (tu.π1).
-
-  - replace (nl (decl_type decl)) with (decl_type (map_decl_anon nl decl));
-      [|destruct decl; reflexivity].
-    constructor. 1: eauto using nlg_wf_local.
-    unfold nlctx. rewrite nth_error_map. now rewrite H.
-  - constructor; eauto using nlg_wf_local.
-    now apply wf_universe_nl.
-  - replace (nl (cst_type decl)) with (cst_type (map_constant_body nl decl));
-      [|destruct decl; reflexivity].
-    constructor; eauto using nlg_wf_local.
-    + unfold declared_constant in *. now erewrite lookup_env_nlg; tea.
-    + red. rewrite global_ext_levels_nlg global_ext_constraints_nlg; assumption.
-  - replace (nl (ind_type idecl)) with (ind_type (nl_one_inductive_body idecl));
-      [|destruct idecl; reflexivity].
-    destruct isdecl as [H1 H2].
-    econstructor; eauto using nlg_wf_local. 1: split.
-    + eapply lookup_env_nlg in H1. eapply H1.
-    + replace (ind_bodies (nl_mutual_inductive_body mdecl)) with
-          (map nl_one_inductive_body (ind_bodies mdecl)); [|now destruct mdecl].
-      rewrite nth_error_map H2. reflexivity.
-    + unfold consistent_instance_ext.
-      rewrite global_ext_levels_nlg global_ext_constraints_nlg; assumption.
-  - cbn.
-    rewrite nl_inds.
-    eapply type_Construct with (idecl0:=nl_one_inductive_body idecl)
-                               (mdecl0:=nl_mutual_inductive_body mdecl)
-                               (cdecl0:=nl_constructor_body cdecl);
-    eauto using nlg_wf_local.
-    + destruct isdecl as [[H1 H2] H3]. repeat split.
-      * eapply lookup_env_nlg in H1. eapply H1.
-      * replace (ind_bodies (nl_mutual_inductive_body mdecl)) with
-            (map nl_one_inductive_body (ind_bodies mdecl)); [|now destruct mdecl].
-        rewrite nth_error_map H2. reflexivity.
-      * rewrite nth_error_map H3. reflexivity.
-    + unfold consistent_instance_ext.
-      rewrite global_ext_levels_nlg global_ext_constraints_nlg; assumption.
-  - rewrite nl_mkApps map_app nl_it_mkLambda_or_LetIn /predctx nl_case_predicate_context.
-    eapply type_Case with  (mdecl0:=nl_mutual_inductive_body mdecl)
-                           (idecl0:=nl_one_inductive_body idecl)
-                           (p0:=nl_predicate nl p); tea; rewrite - ?nl_case_predicate_context.
-    + destruct isdecl as [HH1 HH2]. split.
-      * eapply lookup_env_nlg in HH1. eapply HH1.
-      * replace (ind_bodies (nl_mutual_inductive_body mdecl)) with
-            (map nl_one_inductive_body (ind_bodies mdecl)); [|now destruct mdecl].
-        rewrite nth_error_map HH2. reflexivity.
-    + simpl. clear -X1. move: X1.
-      rewrite /ind_predicate_context.
-      intros a; depelim a. rewrite H. simpl.
-      constructor; auto.
-      * depelim c; constructor; simpl; auto. subst T.
-        rewrite nl_mkApps /=. f_equal.
-        now rewrite nl_to_extended_list nlctx_app_context nlctx_smash_context nl_expand_lets_ctx.
-      * rewrite -nl_expand_lets_ctx. eapply All2_map, (All2_impl a).
-        intros ?? []; constructor; subst; auto.
-    + destruct H0 as [wfpars wfpctx].
-      split; simpl; rewrite ?map_length //.
-      clear -wfpctx. depelim wfpctx.
-      rewrite nl_forget_types H0 /=.
-      simpl. constructor => //.
-      eapply Forall2_map; solve_all.
-    + simpl. tas.
-      unfold consistent_instance_ext.
-      rewrite global_ext_levels_nlg global_ext_constraints_nlg; assumption.
-    + rewrite -nlctx_app_context. exact X4.
-    + now rewrite -nlctx_app_context.
-    + now apply nl_is_allowed_elimination.
-    + revert X6. simpl.
-      rewrite -map_app -nlctx_app_context.
-      rewrite -nlctx_subst_instance.
-      rewrite -[List.rev (nlctx _)]map_rev.
-      clear. induction 1; simpl; constructor; eauto.
-      * now rewrite -(nl_subst_telescope [i] 0 Δ).
-      * now rewrite -(nl_subst_telescope [b] 0 Δ).
-    + now rewrite nl_mkApps map_app in X8.
-    + now eapply nl_wf_branches.
-    + eapply All2i_map, (All2i_impl X9).
-      intros i cdecl br.
-      set (cbt := case_branch_type _ _ _ _ _ _ _ _) in *.
-      intros (convctx & wfctx & bbodyty & IHbody & bty & IHbty).
-      simpl preturn. rewrite -nl_it_mkLambda_or_LetIn.
-      cbn -[case_branch_type].
-      rewrite nl_case_branch_type.
-      rewrite -/cbt. unfold map_pair. cbn.
-      repeat split.
-      * cbn. rewrite -nl_cstr_branch_context.
-        eapply All2_map, (All2_impl convctx).
-        intros ??[]; constructor; subst; auto.
-      * now rewrite -[_ ++ _]nlctx_app_context.
-      * now rewrite - ![_ ++ _]nlctx_app_context.
-      * rewrite - ![_ ++ _]nlctx_app_context. eauto.
-  - destruct pdecl as [pdecl1 pdecl2]; simpl.
-    rewrite map_rev.
-    eapply type_Proj with (mdecl0:=nl_mutual_inductive_body mdecl)
-                          (idecl0:=nl_one_inductive_body idecl)
-                          (cdecl0:=nl_constructor_body cdecl)
-                          (pdecl:=(pdecl1, nl pdecl2)).
-    + destruct isdecl as [[[H1 H2] H3] [H4 H5]]. repeat split.
-      * eapply lookup_env_nlg in H1. eapply H1.
-      * replace (ind_bodies (nl_mutual_inductive_body mdecl)) with
-            (map nl_one_inductive_body (ind_bodies mdecl)); [|now destruct mdecl].
-        rewrite nth_error_map H2. reflexivity.
-      * rewrite nth_error_map H3. reflexivity.
-      * rewrite nth_error_map H4. reflexivity.
-      * assumption.
-    + now rewrite nl_mkApps in X2.
-    + now rewrite map_length.
-  - replace (nl (dtype decl)) with (dtype (map_def_anon nl nl decl));
-      [|destruct decl; reflexivity].
-    assert (XX: nlctx Γ ,,, fix_context (map (map_def_anon nl nl) mfix)
-                = nlctx (Γ ,,, fix_context mfix))
-      by now rewrite <- nl_fix_context, <- nlctx_app_context.
-    constructor.
-    + now eapply fix_guard_nl.
-    + now rewrite nth_error_map H0.
-    + rewrite nlctx_app_context in X. now eapply wf_local_app_inv in X.
-    + clear -X0.
-      apply All_map. eapply All_impl; tea.
-      simpl. intros x [s Hs]. now exists s.
-    + apply All_map. eapply All_impl; tea.
-      simpl. intros [] [s Hs].
-      simpl in *; intuition auto.
-      * rewrite fix_context_length map_length.
-        rewrite fix_context_length in Hs.
-        now rewrite -> XX, <- nl_lift.
-    + now rewrite <-nl_wf_fixpoint.
-  - replace (nl (dtype decl)) with (dtype (map_def_anon nl nl decl));
-      [|destruct decl; reflexivity].
-    assert (XX: nlctx Γ ,,, fix_context (map (map_def_anon nl nl) mfix)
-                = nlctx (Γ ,,, fix_context mfix))
-      by now rewrite <- nl_fix_context, <- nlctx_app_context.
-    constructor; auto.
-    + now apply cofix_guard_nl.
-    + now rewrite nth_error_map H0.
-    + now rewrite nlctx_app_context in X; apply wf_local_app_inv in X.
-    + clear -X0.
-      apply All_map. eapply All_impl; tea.
-      simpl. intros x [s Hs]. now exists s.
-    + apply All_map. eapply All_impl; tea.
-      simpl. intros [] [s Hs].
-      simpl in *; intuition auto.
-      * rewrite fix_context_length map_length.
-        rewrite fix_context_length in Hs.
-        now rewrite -> XX, <- nl_lift.
-    + now rewrite <-nl_wf_cofixpoint.
-  - econstructor; tea.
-    now apply nl_cumul.
-Qed.
 
 (* Corollary reflect_nleq_term : *)
 (*   forall t t', *)
