pcuic/theories/Conversion/PCUICUnivSubstitutionConv.v
@@ -3,7 +3,8 @@ From Coq Require Import ssreflect CRelationClasses.
 From MetaCoq.Template Require Import utils config Universes uGraph.
 From MetaCoq.PCUIC Require Import PCUICAst PCUICAstUtils PCUICInduction
      PCUICLiftSubst PCUICEquality PCUICUnivSubst
-     PCUICCases PCUICContextRelation PCUICTyping PCUICWeakeningEnv
+     PCUICCases PCUICContextRelation PCUICCumulativity PCUICTyping
+     PCUICReduction PCUICWeakeningEnvConv
      PCUICClosed PCUICPosition PCUICGuardCondition.
 
 Require Import Equations.Prop.DepElim.
@@ -520,7 +521,6 @@ Qed.
 
 Definition wf_ext_wk  {cf : checker_flags} (Σ : global_env_ext)
   := wf Σ.1 × on_udecl_prop Σ.1 Σ.2.
-
 
 Lemma not_var_global_ext_levels {cf : checker_flags} Σ φ (hΣ : wf_ext_wk (Σ, Monomorphic_ctx φ)) :
   LS.For_all (negb ∘ Level.is_var)
@@ -1474,48 +1474,6 @@ Proof.
   - econstructor 3. 1: eauto. eapply red1_subst_instance; cbn; eauto.
 Qed.
 
-Lemma conv_decls_subst_instance {cf : checker_flags} (Σ : global_env_ext) {Γ Γ'} u univs d d' :
-  valid_constraints (global_ext_constraints (Σ.1, univs))
-    (subst_instance_cstrs u Σ) ->
-  conv_decls Σ Γ Γ' d d' ->
-  conv_decls (Σ.1, univs) (subst_instance u Γ) (subst_instance u Γ')
-    (subst_instance u d) (subst_instance u d').
-Proof.
-  intros valid Hd; depelim Hd; constructor; tas;
-    eapply subst_instance_equality; tea.
-Qed.
-
-Lemma cumul_decls_subst_instance {cf : checker_flags} (Σ : global_env_ext) {Γ Γ'} u univs d d' :
-  valid_constraints (global_ext_constraints (Σ.1, univs))
-    (subst_instance_cstrs u Σ) ->
-  cumul_decls Σ Γ Γ' d d' ->
-  cumul_decls (Σ.1, univs) (subst_instance u Γ) (subst_instance u Γ')
-    (subst_instance u d) (subst_instance u d').
-Proof.
-  intros valid Hd; depelim Hd; constructor; tas;
-    (eapply subst_instance_equality || eapply cumul_subst_instance); tea.
-Qed.
-
-Lemma conv_ctx_subst_instance {cf : checker_flags} (Σ : global_env_ext) {Γ Γ'} u univs :
-  valid_constraints (global_ext_constraints (Σ.1, univs)) (subst_instance_cstrs u Σ) ->
-  conv_context Σ Γ Γ' ->
-  conv_context (Σ.1, univs) (subst_instance u Γ) (subst_instance u Γ').
-Proof.
-  intros valid.
-  intros; eapply All2_fold_map, All2_fold_impl; tea => ? ? d d'.
-  now eapply conv_decls_subst_instance.
-Qed.
-
-Lemma subst_instance_context_equality_rel {cf : checker_flags} (Σ : global_env_ext) {Γ Γ'} u univs :
-  valid_constraints (global_ext_constraints (Σ.1, univs)) (subst_instance_cstrs u Σ) ->
-  cumul_context Σ Γ Γ' ->
-  cumul_context (Σ.1, univs) (subst_instance u Γ) (subst_instance u Γ').
-Proof.
-  intros valid.
-  intros; eapply All2_fold_map, All2_fold_impl; tea => ? ? d d'.
-  now eapply cumul_decls_subst_instance.
-Qed.
-
 Lemma is_allowed_elimination_subst_instance {cf : checker_flags} (Σ : global_env_ext) univs inst u al :
   valid_constraints (global_ext_constraints (Σ.1, univs))
                     (subst_instance_cstrs inst Σ) ->
@@ -1731,196 +1689,6 @@ Proof.
     + now apply not_var_global_levels in Hl.
 Qed.
 
-Lemma typing_subst_instance {cf : checker_flags} :
-  env_prop (fun Σ Γ t T => forall u univs,
-                wf_ext_wk Σ ->
-                sub_context_set (monomorphic_udecl Σ.2)
-                                (global_ext_context_set (Σ.1, univs)) ->
-                consistent_instance_ext (Σ.1, univs) Σ.2 u ->
-                (Σ.1,univs) ;;; subst_instance u Γ
-                |- subst_instance u t : subst_instance u T)
-          (fun Σ Γ => forall u univs,
-          wf_ext_wk Σ ->
-          sub_context_set (monomorphic_udecl Σ.2)
-                          (global_ext_context_set (Σ.1, univs)) ->
-          consistent_instance_ext (Σ.1, univs) Σ.2 u ->
-          wf_local(Σ.1,univs) (subst_instance u Γ)).
-Proof.
-  apply typing_ind_env; intros Σ wfΣ Γ wfΓ; cbn  -[Universe.make] in *.
-  - rewrite /subst_instance /=.
-    induction 1.
-    + constructor.
-    + simpl. constructor; auto.
-      exists (subst_instance_univ u tu.π1). eapply p; auto.
-    + simpl. constructor; auto.
-      ++ exists (subst_instance_univ u tu.π1). eapply p0; auto.
-      ++ apply p; auto.
-
-  - intros n decl eq X u univs wfΣ' H Hsub. rewrite subst_instance_lift.
-    rewrite map_decl_type. econstructor; aa.
-    unfold subst_instance, map_context.
-    now rewrite nth_error_map eq.
-  - intros l X Hl u univs wfΣ' HSub H.
-    rewrite subst_instance_univ_super.
-    + econstructor.
-      * aa.
-      * now apply wf_universe_subst_instance.
-  - intros n t0 b s1 s2 X X0 X1 X2 X3 u univs wfΣ' HSub H.
-    rewrite product_subst_instance; aa. econstructor.
-    + eapply X1; eauto.
-    + eapply X3; eauto.
-  - intros n t0 b s1 bty X X0 X1 X2 X3 u univs wfΣ' HSub H.
-    econstructor.
-    + eapply X1; aa.
-    + eapply X3; aa.
-  - intros n b b_ty b' s1 b'_ty X X0 X1 X2 X3 X4 X5 u univs wfΣ' HSub H.
-    econstructor; eauto. eapply X5; aa.
-  - intros t0 na A B s u X X0 X1 X2 X3 X4 X5 u0 univs wfΣ' HSub H.
-    rewrite subst_instance_subst. cbn. econstructor.
-    + eapply X1; eauto.
-    + eapply X3; eauto.
-    + eapply X5; eauto.
-  - intros. rewrite subst_instance_two. econstructor; [aa|aa|].
-    clear X X0; cbn in *.
-    eapply consistent_ext_trans; eauto.
-  - intros. rewrite subst_instance_two. econstructor; [aa|aa|].
-    clear X X0; cbn in *.
-    eapply consistent_ext_trans; eauto.
-  - intros. eapply meta_conv. 1: econstructor; aa.
-    clear.
-    unfold type_of_constructor; cbn.
-    rewrite subst_instance_subst. f_equal.
-    + unfold inds. induction #|ind_bodies mdecl|. 1: reflexivity.
-      cbn. now rewrite IHn.
-    + symmetry; apply subst_instance_two.
-
-  - intros ci p c brs args u mdecl idecl isdecl hΣ hΓ indnp eqpctx wfp cup
-      wfpctx pty Hpty Hcpc kelim
-      Hctxi IHctxi Hc IHc notCoFinite wfbrs hbrs i univs wfext Hsub cu.
-    rewrite subst_instance_mkApps subst_instance_it_mkLambda_or_LetIn map_app.
-    cbn.
-    change (subst_instance i (preturn p)) with (preturn (subst_instance i p)).
-    change (subst_instance i (pcontext p)) with (pcontext (subst_instance i p)).
-    change (map_predicate _ _ _ _ _) with (subst_instance i p).
-    rewrite subst_instance_case_predicate_context.
-    eapply type_Case with (p0:=subst_instance i p)
-                          (ps:=subst_instance_univ i u); eauto with pcuic.
-    + simpl. eapply consistent_ext_trans; tea.
-    + now rewrite -subst_instance_case_predicate_context -subst_instance_app_ctx.
-    + rewrite -subst_instance_case_predicate_context - !subst_instance_app_ctx.
-      eapply Hpty; eauto.
-    + destruct Hsub.
-      cbn in *.
-      eapply is_allowed_elimination_subst_instance; aa.
-    + move: IHctxi. simpl.
-      rewrite -subst_instance_app.
-      rewrite -subst_instance_two_context.
-      rewrite -[List.rev (subst_instance i _)]map_rev.
-      clear -wfext Hsub cu. induction 1; cbn; constructor; simpl; eauto.
-      all:now rewrite -(subst_instance_subst_telescope i [_]).
-    + eapply IHc in cu => //.
-      now rewrite subst_instance_mkApps map_app in cu.
-    + rewrite -{1}(map_id (ind_ctors idecl)).
-      eapply All2i_map. eapply All2i_impl; eauto. 
-      cbn -[case_branch_type case_branch_context subst_instance].
-      intros k cdecl br [hctx [hbod [hcbctx [ihbod [hbty ihbty]]]]].
-      rewrite case_branch_type_fst.
-      rewrite - !subst_instance_case_branch_context - !subst_instance_app_ctx.
-      rewrite -subst_instance_case_predicate_context subst_instance_case_branch_type.
-      repeat split; auto.
-      * specialize (ihbod i univs wfext Hsub cu).
-        cbn. eapply ihbod.
-      * specialize (ihbty i univs wfext Hsub cu).
-        cbn. eapply ihbty.
-  - intros p c u mdecl idecl cdecl pdecl isdecl args X X0 X1 X2 H u0 univs wfΣ' HSub H0.
-    rewrite subst_instance_subst. cbn.
-    rewrite !subst_instance_two.
-    rewrite {4}/subst_instance /subst_instance_list /=.
-    rewrite map_rev.
-    econstructor; eauto. 2:now rewrite map_length.
-    eapply X2 in H0; tas. rewrite subst_instance_mkApps in H0.
-    eassumption.
-
-  - intros mfix n decl H H0 H1 X X0 wffix u univs wfΣ' HSub.
-    rewrite (map_dtype _ (subst_instance u)). econstructor.
-    + now eapply fix_guard_subst_instance.
-    + rewrite nth_error_map H0. reflexivity.
-    + specialize (H1 u univs wfΣ' HSub H2).
-      rewrite subst_instance_app in H1.
-      now eapply wf_local_app_inv in H1 as [].
-    + apply All_map, (All_impl X); simpl; intuition auto.
-      destruct X1 as [s Hs]. exists (subst_instance_univ u s).
-      now apply Hs.
-    + eapply All_map, All_impl; tea.
-      intros x [X1 X3]. 
-      specialize (X3 u univs wfΣ' HSub H2). 
-      rewrite (map_dbody (subst_instance u)) in X3.
-      rewrite subst_instance_lift in X3.
-      rewrite fix_context_length ?map_length in X0, X1, X3.
-      rewrite (map_dtype _ (subst_instance u) x) in X3.
-      rewrite subst_instance_app in X3.
-      rewrite <- (fix_context_subst_instance u mfix). len.
-      eapply X3.
-    + red; rewrite <- wffix.
-      unfold wf_fixpoint.
-      rewrite map_map_compose.
-      now rewrite subst_instance_check_one_fix.
-
-  - intros mfix n decl guard H X X0 X1 wfcofix u univs wfΣ' HSub H1.
-    rewrite (map_dtype _ (subst_instance u)). econstructor; tas.
-    + now eapply cofix_guard_subst_instance.
-    + rewrite nth_error_map H. reflexivity.
-    + specialize (X u univs wfΣ' HSub H1).
-      rewrite subst_instance_app in X.
-      now eapply wf_local_app_inv in X as [].
-    + apply All_map, (All_impl X0); simpl; intuition auto.
-      destruct X2 as [s Hs]. exists (subst_instance_univ u s).
-      now apply Hs.
-    + eapply All_map, All_impl; tea.
-      intros x [X1' X3].
-      * specialize (X3 u univs wfΣ' HSub H1). 
-        rewrite (map_dbody (subst_instance u)) in X3.
-        rewrite subst_instance_lift in X3.
-        rewrite fix_context_length ?map_length in X0, X1, X3.
-        rewrite subst_instance_app in X3.
-        rewrite <- (fix_context_subst_instance u mfix).
-        rewrite <- map_dtype. len. eapply X3.
-    + red; rewrite <- wfcofix.
-      unfold wf_cofixpoint.
-      rewrite map_map_compose.
-      now rewrite subst_instance_check_one_cofix.
-      
-  - intros t0 A B X X0 X1 X2 X3 X4 cum u univs wfΣ' HSub H.
-    econstructor.
-    + eapply X2; aa.
-    + eapply X4; aa.
-    + destruct HSub. eapply cumul_subst_instance; aa.
-Qed.
-
-Lemma typing_subst_instance' {cf : checker_flags} Σ φ Γ t T u univs :
-  wf_ext_wk (Σ, univs) ->
-  (Σ, univs) ;;; Γ |- t : T ->
-  sub_context_set (monomorphic_udecl univs) (global_ext_context_set (Σ, φ)) ->
-  consistent_instance_ext (Σ, φ) univs u ->
-  (Σ, φ) ;;; subst_instance u Γ
-            |- subst_instance u t : subst_instance u T.
-Proof.
-  intros X X0 X1.
-  eapply (typing_subst_instance (Σ, univs)); tas. apply X.
-Qed.
-
-Lemma typing_subst_instance_wf_local {cf : checker_flags} Σ φ Γ u univs :
-  wf_ext_wk (Σ, univs) ->
-  wf_local (Σ, univs) Γ ->
-  sub_context_set (monomorphic_udecl univs) (global_ext_context_set (Σ, φ)) ->
-  consistent_instance_ext (Σ, φ) univs u ->
-  wf_local (Σ, φ) (subst_instance u Γ).
-Proof.
-  intros X X0 X1.
-  eapply (env_prop_wf_local typing_subst_instance (Σ, univs)); tas. 1: apply X.
-Qed.
-
-
 Definition global_context_set Σ : ContextSet.t
   := (global_levels Σ, global_constraints Σ).
 
@@ -1947,127 +1715,10 @@ Proof.
     [apply LevelSetProp.subset_empty|apply ConstraintSetProp.subset_empty].
 Qed.
 
-
-Lemma typing_subst_instance'' {cf : checker_flags} Σ φ Γ t T u univs :
-  wf_ext_wk (Σ, univs) ->
-  (Σ, univs) ;;; Γ |- t : T ->
-  sub_context_set (monomorphic_udecl univs) (global_context_set Σ) ->
-  consistent_instance_ext (Σ, φ) univs u ->
-  (Σ, φ) ;;; subst_instance u Γ
-            |- subst_instance u t : subst_instance u T.
-Proof.
-  intros X X0 X1.
-  eapply (typing_subst_instance (Σ, univs)); tas. 1: apply X.
-  etransitivity; tea. apply global_context_set_sub_ext.
-Qed.
-
-Lemma typing_subst_instance_ctx {cf : checker_flags} (Σ : global_env_ext) Γ t T ctx u :
-  wf Σ.1 ->
-  on_udecl_prop Σ (Polymorphic_ctx ctx) ->
-  (Σ.1, Polymorphic_ctx ctx) ;;; Γ |- t : T ->
-  consistent_instance_ext Σ (Polymorphic_ctx ctx) u ->
-  Σ ;;; subst_instance u Γ
-            |- subst_instance u t : subst_instance u T.
-Proof.
-  destruct Σ as [Σ φ]. intros X X0 X1.
-  eapply typing_subst_instance''; tea.
-  - split; tas.
-  - simpl. unfold sub_context_set. split; simpl.
-    * intros x hx. now eapply LS.empty_spec in hx.
-    * intros x hx. now eapply CS.empty_spec in hx. 
-Qed.
-
-Lemma typing_subst_instance_decl  {cf : checker_flags}Σ Γ t T c decl u :
-  wf Σ.1 ->
-  lookup_env Σ.1 c = Some decl ->
-  (Σ.1, universes_decl_of_decl decl) ;;; Γ |- t : T ->
-  consistent_instance_ext Σ (universes_decl_of_decl decl) u ->
-  Σ ;;; subst_instance u Γ
-            |- subst_instance u t : subst_instance u T.
-Proof.
-  destruct Σ as [Σ φ]. intros X X0 X1 X2.
-  eapply typing_subst_instance''; tea.
-  - split; tas.
-    eapply weaken_lookup_on_global_env'; tea.
-  - eapply weaken_lookup_on_global_env''; tea.
-Qed.
-
-Lemma wf_local_instantiate_poly {cf : checker_flags} {Σ ctx Γ u} : 
-  wf_ext (Σ.1, Polymorphic_ctx ctx) ->
-  consistent_instance_ext Σ (Polymorphic_ctx ctx) u ->
-  wf_local (Σ.1, Polymorphic_ctx ctx) Γ -> 
-  wf_local Σ (subst_instance u Γ).
-Proof.
-  intros wfΣ Huniv wf.
-  epose proof (type_Sort _ _ Universes.Universe.lProp wf) as ty. forward ty.
-  - now simpl.
-  - eapply typing_subst_instance_ctx in ty;   
-    eauto using typing_wf_local. 
-    * apply wfΣ.
-    * destruct wfΣ. now eapply on_udecl_on_udecl_prop.
-Qed.
-
-Lemma wf_local_instantiate {cf : checker_flags} {Σ} {decl : global_decl} {Γ u c} : 
-  wf Σ.1 ->
-  lookup_env Σ.1 c = Some decl ->
-  consistent_instance_ext Σ (universes_decl_of_decl decl) u ->
-  wf_local (Σ.1, universes_decl_of_decl decl) Γ -> 
-  wf_local Σ (subst_instance u Γ).
-Proof.
-  intros wfΣ Hdecl Huniv wf.
-  epose proof (type_Sort _ _ Universes.Universe.lProp wf) as ty. forward ty.
-  - now simpl.
-  - eapply typing_subst_instance_decl in ty;   
-    eauto using typing_wf_local.
-Qed.
-
-Lemma isType_subst_instance_decl {cf : checker_flags} Σ Γ T c decl u :
-  wf Σ.1 ->
-  lookup_env Σ.1 c = Some decl ->
-  isType (Σ.1, universes_decl_of_decl decl) Γ T ->
-  consistent_instance_ext Σ (universes_decl_of_decl decl) u ->
-  isType Σ (subst_instance u Γ) (subst_instance u T).
-Proof.
-  intros wfΣ look [s Hs] cu.
-  exists (subst_instance u s). 
-  now eapply (typing_subst_instance_decl _ _ _ (tSort _)).
-Qed.
-
-Definition wf_global_ext {cf : checker_flags} Σ ext :=
+Definition wf_global_ext Σ ext :=
   (wf_ext_wk (Σ, ext) * sub_context_set (monomorphic_udecl ext) (global_context_set Σ))%type.
 
-Lemma wf_local_subst_instance {cf : checker_flags} Σ Γ ext u :
-  wf_global_ext Σ.1 ext ->
-  consistent_instance_ext Σ ext u ->
-  wf_local (Σ.1, ext) Γ ->
-  wf_local Σ (subst_instance u Γ).
-Proof.
-  destruct Σ as [Σ φ]. intros X X0 X1. simpl in *.
-  induction X1; cbn; constructor; auto.
-  - destruct t0 as [s Hs]. hnf.
-    eapply typing_subst_instance'' in Hs; eauto; apply X.
-  - destruct t0 as [s Hs]. hnf.
-    eapply typing_subst_instance'' in Hs; eauto; apply X.
-  - hnf in t1 |- *.
-    eapply typing_subst_instance'' in t1; eauto; apply X.
-Qed.
-
-Lemma wf_local_subst_instance_decl {cf : checker_flags} Σ Γ c decl u :
-  wf Σ.1 ->
-  lookup_env Σ.1 c = Some decl ->
-  wf_local (Σ.1, universes_decl_of_decl decl) Γ ->
-  consistent_instance_ext Σ (universes_decl_of_decl decl) u ->
-  wf_local Σ (subst_instance u Γ).
-Proof.
-  destruct Σ as [Σ φ]. intros X X0 X1 X2.
-  induction X1; cbn; constructor; auto.
-  - destruct t0 as [s Hs]. hnf.
-    eapply typing_subst_instance_decl in Hs; eauto.
-  - destruct t0 as [s Hs]. hnf.
-    eapply typing_subst_instance_decl in Hs; eauto.
-  - hnf in t1 |- *.
-    eapply typing_subst_instance_decl in t1; eauto.
-Qed.
+End CheckerFlags.
 
 Require Import Morphisms.
 Require Import ssreflect.
@@ -2075,13 +1726,6 @@ Set SimplIsCbn.
 
 Section SubstIdentity.
   Context `{cf:checker_flags}.
-
-  Lemma mapi_nth {A B} (l : list A) (l' : list B) (default : A) : #|l| = #|l'| ->
-    mapi (fun i _ => nth i l default) l' = l.
-  Proof.
-    induction l' in l |- *; destruct l => /= //.
-    simpl. intros [= Hl]. f_equal. now rewrite mapi_rec_Sk.
-  Qed.
 
   Lemma subst_instance_id_mdecl Σ u mdecl :
     consistent_instance_ext Σ (ind_universes mdecl) u ->
@@ -2416,54 +2060,6 @@ Section SubstIdentity.
   Proof.
     intros. eapply (env_prop_wf_local subst_abstract_instance_id) in X0; eauto.
     apply X.
-  Qed.
-
-  Lemma subst_instance_ind_sort_id Σ mdecl ind idecl :
-    wf Σ ->
-    declared_inductive Σ ind mdecl idecl ->
-    let u := abstract_instance (ind_universes mdecl) in
-    subst_instance_univ u (ind_sort idecl) = ind_sort idecl.
-  Proof.
-    intros wfΣ decli u.
-    pose proof (on_declared_inductive decli) as [onmind oib].
-    pose proof (onArity oib) as ona.
-    rewrite (oib.(ind_arity_eq)) in ona.
-    red in ona. destruct ona.
-    eapply typed_subst_abstract_instance in t.
-    2:split; simpl; auto.
-    - rewrite !subst_instance_it_mkProd_or_LetIn in t.
-      eapply (f_equal (destArity [])) in t.
-      rewrite !destArity_it_mkProd_or_LetIn in t. simpl in t. noconf t.
-      simpl in H; noconf H. apply H0.
-    - destruct decli as [declm _].
-      eapply declared_inductive_wf_global_ext in declm; auto.
-      destruct declm. apply w.
-  Qed.
-
-  Lemma subst_instance_ind_type_id Σ mdecl ind idecl :
-    wf Σ ->
-    declared_inductive Σ ind mdecl idecl ->
-    let u := abstract_instance (ind_universes mdecl) in
-    subst_instance u (ind_type idecl) = ind_type idecl.
-  Proof.
-    intros wfΣ decli u.
-    pose proof (on_declared_inductive decli) as [_ oib].
-    pose proof (onArity oib) as ona.
-    rewrite (oib.(ind_arity_eq)) in ona |- *.
-    red in ona. destruct ona.
-    eapply typed_subst_abstract_instance in t; eauto.
-    destruct decli as [declm _].
-    eapply declared_inductive_wf_global_ext in declm; auto.
-    destruct declm. apply w.
-  Qed.
-
-  Lemma isType_subst_instance_id Σ Γ T :
-    wf_ext_wk Σ ->
-    let u := abstract_instance Σ.2 in
-    isType Σ Γ T -> subst_instance u T = T.
-  Proof.
-    intros wf_ext u isT.
-    destruct isT. eapply typed_subst_abstract_instance in t; auto.
   Qed.
 
 End SubstIdentity.
