pcuic/theories/Conversion/PCUICWeakeningEnvConv.v
@@ -2,7 +2,8 @@
 From MetaCoq.Template Require Import config utils.
 From MetaCoq.PCUIC Require Import PCUICAst PCUICAstUtils
   PCUICEquality PCUICContextSubst PCUICUnivSubst PCUICCases
-  PCUICTyping PCUICGuardCondition PCUICContextRelation PCUICGlobalEnv.
+  PCUICReduction PCUICCumulativity PCUICTyping
+  PCUICGuardCondition PCUICContextRelation PCUICGlobalEnv.
 From Equations Require Import Equations.
 
 Require Import ssreflect.
@@ -326,8 +327,8 @@ Qed.
 Lemma weakening_env_conv `{CF:checker_flags} Σ Σ' φ Γ M N :
   wf Σ' ->
   extends Σ Σ' ->
-  conv (Σ, φ) Γ M N ->
-  conv (Σ', φ) Γ M N.
+  convAlgo (Σ, φ) Γ M N ->
+  convAlgo (Σ', φ) Γ M N.
 Proof.
   intros wfΣ [Σ'' ->].
   induction 1; simpl.
@@ -343,8 +344,8 @@ Qed.
 Lemma weakening_env_cumul `{CF:checker_flags} Σ Σ' φ Γ M N :
   wf Σ' ->
   extends Σ Σ' ->
-  cumul (Σ, φ) Γ M N ->
-  cumul (Σ', φ) Γ M N.
+  cumulAlgo (Σ, φ) Γ M N ->
+  cumulAlgo (Σ', φ) Γ M N.
 Proof.
   intros wfΣ [Σ'' ->].
   induction 1; simpl.
@@ -356,49 +357,6 @@ Proof.
   - econstructor 2; eauto. eapply weakening_env_red1; eauto. exists Σ''; eauto.
   - econstructor 3; eauto. eapply weakening_env_red1; eauto. exists Σ''; eauto.
 Qed.
-
-Lemma weakening_env_conv_decls {cf} {Σ φ Σ' Γ Γ'} :
-  wf Σ' -> extends Σ Σ' ->
-  CRelationClasses.subrelation (conv_decls (Σ, φ) Γ Γ') (conv_decls (Σ', φ) Γ Γ').
-Proof.
-  intros wf ext d d' Hd; depelim Hd; constructor; tas;
-    eapply weakening_env_conv; tea.
-Qed.
-
-Lemma weakening_env_cumul_decls {cf} {Σ φ Σ' Γ Γ'} :
-  wf Σ' -> extends Σ Σ' ->
-  CRelationClasses.subrelation (cumul_decls (Σ, φ) Γ Γ') (cumul_decls (Σ', φ) Γ Γ').
-Proof.
-  intros wf ext d d' Hd; depelim Hd; constructor; tas;
-    (eapply weakening_env_conv || eapply weakening_env_cumul); tea.
-Qed.
-
-Lemma weakening_env_conv_ctx {cf} {Σ Σ' φ Γ Δ} :
-  wf Σ' ->
-  extends Σ Σ' ->
-  conv_context (Σ, φ) Γ Δ ->
-  conv_context (Σ', φ) Γ Δ.
-Proof.
-  intros wf ext.
-  intros; eapply All2_fold_impl; tea => Γ0 Γ' d d'.
-  now eapply weakening_env_conv_decls.
-Qed.
-
-#[global]
-Hint Resolve weakening_env_conv_ctx : extends.
-
-Lemma weakening_env_cumul_ctx {cf} {Σ Σ' φ Γ Δ} :
-  wf Σ' ->
-  extends Σ Σ' ->
-  cumul_context (Σ, φ) Γ Δ ->
-  cumul_context (Σ', φ) Γ Δ.
-Proof.
-  intros wf ext.
-  intros; eapply All2_fold_impl; tea => Γ0 Γ' d d'.
-  now eapply weakening_env_cumul_decls.
-Qed.
-#[global]
-Hint Resolve weakening_env_cumul_ctx : extends.
 
 Lemma weakening_env_is_allowed_elimination `{CF:checker_flags} Σ Σ' φ u allowed :
   wf Σ' -> extends Σ Σ' ->
@@ -414,6 +372,7 @@ Proof.
     apply global_ext_constraints_app. }
   destruct allowed; auto; cbn in *; destruct ?; auto.
 Qed.
+
 #[global]
 Hint Resolve weakening_env_is_allowed_elimination : extends.
 
@@ -523,242 +482,7 @@ Qed.
 #[global]
 Hint Resolve extends_wf_fixpoint extends_wf_cofixpoint : extends.
 
-Lemma weakening_env `{checker_flags} :
-  env_prop (fun Σ Γ t T =>
-              forall Σ', wf Σ' -> extends Σ.1 Σ' -> (Σ', Σ.2) ;;; Γ |- t : T)
-           (fun Σ Γ =>
-             forall Σ', wf Σ' -> extends Σ.1 Σ' -> wf_local (Σ', Σ.2) Γ).
-Proof.
-  apply typing_ind_env; intros;
-    rename_all_hyps; try solve [econstructor; eauto 2 with extends].
 
-  - induction X; constructor; eauto 2 with extends.
-    + eexists; eapply p; eauto.
-    + eexists; eapply p0; eauto.
-    + eapply p; eauto.
-  - econstructor; eauto 2 with extends.
-    now apply extends_wf_universe.
-  - econstructor; eauto 2 with extends.
-    * revert X6. clear -Σ' wfΣ' extΣ.
-      induction 1; constructor; eauto with extends.
-    * close_Forall. intros; intuition eauto with extends.
-  - econstructor; eauto with extends.
-    + eapply fix_guard_extends; eauto.
-    + specialize (forall_Σ' _ wfΣ' extΣ).
-      now apply wf_local_app_inv in forall_Σ'.
-    + eapply (All_impl X0); simpl; intuition eauto with extends.
-      destruct X as [s Hs]; exists s. intuition eauto with extends.
-    + eapply All_impl; eauto; simpl; intuition eauto with extends.
-  - econstructor; eauto with extends.
-    + eapply cofix_guard_extends; eauto.
-    + specialize (forall_Σ' _ wfΣ' extΣ).
-      now apply wf_local_app_inv in forall_Σ'.
-    + eapply (All_impl X0); simpl; intuition eauto with extends.
-      destruct X as [s Hs]; exists s. intuition eauto with extends.
-    + eapply All_impl; eauto; simpl; intuition eauto with extends.
-  - econstructor. 1: eauto.
-    + eapply forall_Σ'1; eauto.
-    + destruct Σ as [Σ φ]. eapply weakening_env_cumul in cumulA; eauto.
-Qed.
-
-Definition weaken_env_prop `{checker_flags}
-           (P : global_env_ext -> context -> term -> option term -> Type) :=
-  forall Σ Σ' φ, wf Σ' -> extends Σ Σ' -> forall Γ t T, P (Σ, φ) Γ t T -> P (Σ', φ) Γ t T.
-
-Lemma weakening_on_global_decl `{checker_flags} P Σ Σ' φ kn decl :
-  weaken_env_prop P ->
-  wf Σ' -> extends Σ Σ' ->
-  on_global_decl P (Σ, φ) kn decl ->
-  on_global_decl P (Σ', φ) kn decl.
-Proof.
-  unfold weaken_env_prop.
-  intros HPΣ wfΣ' Hext Hdecl.
-  destruct decl.
-  1:{
-    destruct c. destruct cst_body0.
-    - simpl in *.
-      red in Hdecl |- *. simpl in *.
-      eapply HPΣ; eauto.
-    - eapply HPΣ; eauto.
-  }
-  simpl in *.
-  destruct Hdecl as [onI onP onnP]; constructor; eauto.
-  - eapply Alli_impl; eauto. intros.
-    destruct X. unshelve econstructor; eauto.
-    + unfold on_type in *; intuition eauto.
-    + unfold on_constructors in *. eapply All2_impl; eauto.
-      intros.
-      destruct X as [? ? ? ?]. unshelve econstructor; eauto.
-      * unfold on_type in *; eauto.
-      * clear on_cindices cstr_eq cstr_args_length.
-        revert on_cargs.
-        induction (cstr_args x0) in y |- *; destruct y; simpl in *; eauto.
-        ** destruct a as [na [b|] ty]; simpl in *; intuition eauto.
-        ** destruct a as [na [b|] ty]; simpl in *; intuition eauto.
-      * clear on_ctype on_cargs.
-        revert on_cindices.
-        generalize (List.rev (lift_context #|cstr_args x0| 0 (ind_indices x))).
-        generalize (cstr_indices x0).
-        induction 1; constructor; eauto.
-      * simpl.
-        intros v indv. specialize (on_ctype_variance v indv).
-        simpl in *. move: on_ctype_variance.
-        unfold cstr_respects_variance. destruct variance_universes as [[[univs u] u']|]; auto.
-        intros [args idxs]. split.
-        ** eapply (All2_fold_impl args); intros.
-           inversion X; constructor; auto.
-           ++ eapply weakening_env_cumul; eauto.
-           ++ eapply weakening_env_conv; eauto.
-           ++ eapply weakening_env_cumul; eauto.
-        ** eapply (All2_impl idxs); intros.
-          eapply weakening_env_conv; eauto.
-    + unfold check_ind_sorts in *.
-      destruct Universe.is_prop; auto.
-      destruct Universe.is_sprop; auto.
-      split; [apply fst in ind_sorts|apply snd in ind_sorts].
-      * eapply Forall_impl; tea; cbn.
-        intros. eapply Forall_impl; tea; simpl; intros.
-        eapply leq_universe_subset; tea.
-        apply weakening_env_global_ext_constraints; tea.
-      * destruct indices_matter; [|trivial]. clear -ind_sorts HPΣ wfΣ' Hext.
-        induction ind_indices; simpl in *; auto.
-        -- eapply (extends_wf_universe (Σ:=(Σ,φ)) Σ'); auto.
-        -- destruct a as [na [b|] ty]; simpl in *; intuition eauto.
-    + intros v onv.
-      move: (onIndices v onv). unfold ind_respects_variance.
-      destruct variance_universes as [[[univs u] u']|] => //.
-      intros idx; eapply (All2_fold_impl idx); simpl.
-      intros par par' t t' d.
-      inv d; constructor; auto.
-      ++ eapply weakening_env_cumul; eauto.
-      ++ eapply weakening_env_conv; eauto.
-      ++ eapply weakening_env_cumul; eauto.
-  - red in onP |- *. eapply All_local_env_impl; eauto.
-  - move: onVariance.
-    rewrite /on_variance. destruct ind_universes => //.
-    destruct ind_variance => //.
-    intros [univs' [i [i' []]]]. exists univs', i, i'. split => //.
-    all:eapply weakening_env_consistent_instance; tea.
-Qed.
-
-Lemma weakening_env_lookup_on_global_env `{checker_flags} P Σ Σ' c decl :
-  weaken_env_prop P ->
-  wf Σ' -> extends Σ Σ' -> on_global_env P Σ ->
-  lookup_env Σ c = Some decl ->
-  on_global_decl P (Σ', universes_decl_of_decl decl) c decl.
-Proof.
-  intros HP wfΣ Hext HΣ.
-  induction HΣ; simpl. 1: congruence.
-  assert (HH: extends Σ Σ'). {
-    destruct Hext as [Σ'' HΣ''].
-    exists (Σ'' ++ [(kn, d)]). now rewrite <- app_assoc.
-  }
-  unfold eq_kername; destruct kername_eq_dec; subst.
-  - intros [= ->]. subst.
-    clear Hext; eapply weakening_on_global_decl; eauto.
-  - now apply IHHΣ.
-Qed.
-
-Lemma weaken_lookup_on_global_env `{checker_flags} P Σ c decl :
-  weaken_env_prop P ->
-  wf Σ -> on_global_env P Σ ->
-  lookup_env Σ c = Some decl ->
-  on_global_decl P (Σ, universes_decl_of_decl decl) c decl.
-Proof.
-  intros. eapply weakening_env_lookup_on_global_env; eauto.
-  exists []; simpl; destruct Σ; eauto.
-Qed.
-
-Lemma declared_constant_inv `{checker_flags} Σ P cst decl :
-  weaken_env_prop (lift_typing P) ->
-  wf Σ -> Forall_decls_typing P Σ ->
-  declared_constant Σ cst decl ->
-  on_constant_decl (lift_typing P) (Σ, cst_universes decl) decl.
-Proof.
-  intros.
-  eapply weaken_lookup_on_global_env in X1; eauto. apply X1.
-Qed.
-
-
-Lemma declared_minductive_inv `{checker_flags} {Σ P ind mdecl} :
-  weaken_env_prop (lift_typing P) ->
-  wf Σ -> Forall_decls_typing P Σ ->
-  declared_minductive Σ ind mdecl ->
-  on_inductive (lift_typing P) (Σ, ind_universes mdecl) ind mdecl.
-Proof.
-  intros.
-  eapply weaken_lookup_on_global_env in X1; eauto. apply X1.
-Qed.
-
-Lemma declared_inductive_inv `{checker_flags} {Σ P ind mdecl idecl} :
-  weaken_env_prop (lift_typing P) ->
-  wf Σ -> Forall_decls_typing P Σ ->
-  declared_inductive Σ ind mdecl idecl ->
-  on_ind_body (lift_typing P) (Σ, ind_universes mdecl) (inductive_mind ind) mdecl (inductive_ind ind) idecl.
-Proof.
-  intros.
-  destruct H0 as [Hmdecl Hidecl].
-  eapply declared_minductive_inv in Hmdecl; eauto.
-  apply onInductives in Hmdecl.
-  eapply nth_error_alli in Hidecl; eauto.
-  apply Hidecl.
-Qed.
-
-Lemma declared_constructor_inv `{checker_flags} {Σ P mdecl idecl ref cdecl}
-  (HP : weaken_env_prop (lift_typing P))
-  (wfΣ : wf Σ)
-  (HΣ : Forall_decls_typing P Σ)
-  (Hdecl : declared_constructor Σ ref mdecl idecl cdecl) :
-  ∑ cs,
-  let onib := declared_inductive_inv HP wfΣ HΣ (let (x, _) := Hdecl in x) in
-  nth_error onib.(ind_cunivs) ref.2 = Some cs
-  × on_constructor (lift_typing P) (Σ, ind_universes mdecl) mdecl
-                   (inductive_ind ref.1) idecl idecl.(ind_indices) cdecl cs.
-Proof.
-  intros.
-  destruct Hdecl as [Hidecl Hcdecl].
-  set (declared_inductive_inv HP wfΣ HΣ Hidecl) as HH.
-  clearbody HH. pose proof HH.(onConstructors) as HH'.
-  eapply All2_nth_error_Some in Hcdecl; tea.
-Defined.
-
-Lemma declared_projection_inv `{checker_flags} {Σ P mdecl idecl cdecl ref pdecl} :
-  forall (HP : weaken_env_prop (lift_typing P))
-  (wfΣ : wf Σ)
-  (HΣ : Forall_decls_typing P Σ)
-  (Hdecl : declared_projection Σ ref mdecl idecl cdecl pdecl),
-  match idecl.(ind_ctors) return Type with
-  | [c] =>
-    let oib := declared_inductive_inv HP wfΣ HΣ (let (x, _) := Hdecl in
-      let (x, _) := x in x) in
-    (match oib.(ind_cunivs) with
-     | [cs] => sorts_local_ctx (lift_typing P) (Σ, ind_universes mdecl) (arities_context (ind_bodies mdecl) ,,, ind_params mdecl) (cstr_args c) cs
-     | _ => False
-    end) *
-    on_projections mdecl (inductive_mind ref.1.1) (inductive_ind ref.1.1) idecl (idecl.(ind_indices)) c *
-    ((snd ref) < context_assumptions c.(cstr_args)) *
-    on_projection mdecl (inductive_mind ref.1.1) (inductive_ind ref.1.1) c (snd ref) pdecl
-  | _ => False
-  end.
-Proof.
-  intros.
-  destruct (declared_inductive_inv HP wfΣ HΣ (let (x, _) := Hdecl in let (x, _) := x in x)) in *.
-  destruct Hdecl as [Hidecl [Hcdecl Hnpar]]. simpl.
-  forward onProjections.
-  { eapply nth_error_Some_length in Hcdecl.
-    destruct (ind_projs idecl); simpl in *; try lia. congruence. }
-  destruct (ind_ctors idecl) as [|? []]; try contradiction.
-  destruct ind_cunivs as [|? []]; try contradiction; depelim onConstructors.
-  2:{ depelim onConstructors. }
-  intuition auto.
-  - destruct onProjections.
-    destruct (ind_ctors idecl) as [|? []]; simpl in *; try discriminate.
-    inv onConstructors. now eapply on_cargs in o.
-  - destruct onProjections. eapply nth_error_Some_length in Hcdecl. lia.
-  - destruct onProjections.
-    eapply nth_error_alli in Hcdecl; eauto.
-    eapply Hcdecl.
-Qed.
 
 Lemma wf_extends `{checker_flags} {Σ Σ'} : wf Σ' -> extends Σ Σ' -> wf Σ.
 Proof.
@@ -767,105 +491,7 @@ Proof.
   inv HΣ'. auto.
 Qed.
 
-Lemma weaken_env_prop_typing `{checker_flags} : weaken_env_prop (lift_typing typing).
-Proof.
-  red. intros * wfΣ' Hext *.
-  destruct T; simpl.
-  - intros Ht. pose proof (wf_extends wfΣ' Hext).
-    eapply (weakening_env (_, _)); eauto.
-  - intros [s Ht]. pose proof (wf_extends wfΣ' Hext). exists s.
-    eapply (weakening_env (_, _)); eauto.
-Qed.
 
-#[global]
-Hint Unfold weaken_env_prop : pcuic.
-
-Lemma on_declared_constant `{checker_flags} {Σ cst decl} :
-  wf Σ -> declared_constant Σ cst decl ->
-  on_constant_decl (lift_typing typing) (Σ, cst_universes decl) decl.
-Proof.
-  intros.
-  eapply declared_constant_inv; tea.
-  apply weaken_env_prop_typing.
-Qed.
-
-Lemma weaken_wf_local `{checker_flags} (Σ : global_env_ext) Σ' Γ :
-  extends Σ Σ' -> wf Σ' -> wf_local Σ Γ -> wf_local (Σ', Σ.2) Γ.
-Proof.
-  intros * Hext wfΣ' *.
-  intros wfΓ.
-  eapply (env_prop_wf_local weakening_env); eauto.
-  now eapply wf_extends.
-Qed.
-
-#[global]
-Hint Resolve weaken_wf_local | 100 : pcuic.
-
-Lemma on_declared_minductive `{checker_flags} {Σ ref decl} :
-  wf Σ ->
-  declared_minductive Σ ref decl ->
-  on_inductive (lift_typing typing) (Σ, ind_universes decl) ref decl.
-Proof.
-  intros wfΣ Hdecl.
-  apply (declared_minductive_inv weaken_env_prop_typing wfΣ wfΣ Hdecl).
-Qed.
-
-Lemma on_declared_inductive `{checker_flags} {Σ ref mdecl idecl} {wfΣ : wf Σ} :
-  declared_inductive Σ ref mdecl idecl ->
-  on_inductive (lift_typing typing) (Σ, ind_universes mdecl) (inductive_mind ref) mdecl *
-  on_ind_body (lift_typing typing) (Σ, ind_universes mdecl) (inductive_mind ref) mdecl (inductive_ind ref) idecl.
-Proof.
-  intros Hdecl.
-  split.
-  - destruct Hdecl as [Hmdecl _]. now apply on_declared_minductive in Hmdecl.
-  - apply (declared_inductive_inv weaken_env_prop_typing wfΣ wfΣ Hdecl).
-Defined.
-
-Lemma on_declared_constructor `{checker_flags} {Σ ref mdecl idecl cdecl}
-  {wfΣ : wf Σ}
-  (Hdecl : declared_constructor Σ ref mdecl idecl cdecl) :
-  on_inductive (lift_typing typing) (Σ, ind_universes mdecl)
-               (inductive_mind (fst ref)) mdecl *
-  on_ind_body (lift_typing typing) (Σ, ind_universes mdecl)
-              (inductive_mind (fst ref)) mdecl (inductive_ind (fst ref)) idecl *
-  ∑ ind_ctor_sort,
-    let onib := declared_inductive_inv weaken_env_prop_typing wfΣ wfΣ (let (x, _) := Hdecl in x) in
-     nth_error (ind_cunivs onib) ref.2 = Some ind_ctor_sort
-    ×  on_constructor (lift_typing typing) (Σ, ind_universes mdecl)
-                 mdecl (inductive_ind (fst ref))
-                 idecl idecl.(ind_indices) cdecl ind_ctor_sort.
-Proof.
-  split.
-  - apply (on_declared_inductive Hdecl).
-  - apply (declared_constructor_inv weaken_env_prop_typing wfΣ wfΣ Hdecl).
-Defined.
-
-Lemma on_declared_projection `{checker_flags} {Σ ref mdecl idecl cdecl pdecl} {wfΣ : wf Σ}
-  (Hdecl : declared_projection Σ ref mdecl idecl cdecl pdecl) :
-  on_inductive (lift_typing typing) (Σ, ind_universes mdecl) (inductive_mind (fst (fst ref))) mdecl *
-  (idecl.(ind_ctors) = [cdecl]) *
-  let oib := declared_inductive_inv weaken_env_prop_typing wfΣ wfΣ (let (x, _) := Hdecl in let (x, _) := x in x) in
-  (match oib.(ind_cunivs) with
-  | [cs] => sorts_local_ctx (lift_typing typing) (Σ, ind_universes mdecl)
-      (arities_context (ind_bodies mdecl) ,,, ind_params mdecl) (cstr_args cdecl) cs
-    | _ => False
-  end) *
-  on_projections mdecl (inductive_mind ref.1.1) (inductive_ind ref.1.1) idecl (idecl.(ind_indices)) cdecl *
-  ((snd ref) < context_assumptions cdecl.(cstr_args)) *
-  on_projection mdecl (inductive_mind ref.1.1) (inductive_ind ref.1.1) cdecl (snd ref) pdecl.
-Proof.
-  have hctors : idecl.(ind_ctors) = [cdecl].
-  { pose proof (declared_projection_inv weaken_env_prop_typing wfΣ wfΣ Hdecl).
-    move: X. destruct Hdecl. destruct d. cbn in *.
-    move: e. destruct (ind_ctors idecl) as [|? []] => //.
-    intros [= ->] => //. }
-  split.
-  - split => //.
-    apply (on_declared_inductive Hdecl).
-  - pose proof (declared_projection_inv weaken_env_prop_typing wfΣ wfΣ Hdecl).
-    destruct Hdecl. cbn in *. destruct d; cbn in *.
-    now rewrite hctors in X.
-Qed.
 
 Definition on_udecl_prop `{checker_flags} Σ (udecl : universes_decl)
   := let levels := levels_of_udecl udecl in
@@ -881,6 +507,7 @@ Definition on_udecl_prop `{checker_flags} Σ (udecl : universes_decl)
                                /\ satisfiable_udecl Σ udecl
        | _ => True
        end.
+
 
 Lemma weaken_lookup_on_global_env' `{checker_flags} Σ c decl :
   wf Σ ->
@@ -953,3 +580,7 @@ Lemma on_udecl_on_udecl_prop {cf:checker_flags} Σ ctx :
 Proof.
   intros [? [? [_ ?]]]. red. split; auto.
 Qed.
+
+Definition weaken_env_prop `{checker_flags}
+           (P : global_env_ext -> context -> term -> option term -> Type) :=
+  forall Σ Σ' φ, wf Σ' -> extends Σ Σ' -> forall Γ t T, P (Σ, φ) Γ t T -> P (Σ', φ) Γ t T.
