pcuic/theories/PCUICParallelReduction.v
@@ -3,9 +3,9 @@ Require Import RelationClasses CRelationClasses.
 From MetaCoq.Template Require Import config utils.
 From MetaCoq.PCUIC Require Import PCUICUtils PCUICAst PCUICAstUtils PCUICDepth PCUICCases
      PCUICLiftSubst PCUICUnivSubst PCUICReduction PCUICTyping
-     PCUICSigmaCalculus PCUICWeakeningEnv PCUICInduction
-     PCUICRenameDef PCUICRenameProp PCUICInstDef PCUICInstProp PCUICOnFreeVars
-     PCUICContextRelation PCUICWeakening PCUICSubstitution.
+     PCUICSigmaCalculus PCUICWeakeningEnvConv PCUICInduction
+     PCUICRenameDef PCUICRenameConv PCUICInstDef PCUICInstConv PCUICOnFreeVars PCUICWeakening
+     PCUICContextRelation PCUICSubstitution.
 
 Require Import ssreflect ssrbool.
 From Equations Require Import Equations.
@@ -429,7 +429,7 @@ Section ParallelReduction.
     | pred1_ctx _ _ ?G => fresh "pred" G
     | nat -> bool => fresh "P"
     | nat -> nat => fresh "f"
-    | _ => PCUICWeakeningEnv.my_rename_hyp h th
+    | _ => PCUICWeakeningEnvConv.my_rename_hyp h th
     end.
 
   Ltac rename_hyp h ht ::= my_rename_hyp h ht.
@@ -922,7 +922,7 @@ Ltac my_rename_hyp h th :=
   | nat -> bool => fresh "P"
   | nat -> nat => fresh "f"
   | urenaming _ _ _ ?f => fresh "u" f
-  | _ => PCUICWeakeningEnv.my_rename_hyp h th
+  | _ => PCUICWeakeningEnvConv.my_rename_hyp h th
   end.
 
 Ltac rename_hyp h ht ::= my_rename_hyp h ht.
@@ -1352,7 +1352,7 @@ Qed.
     - rewrite rename_subst_instance.
       econstructor; tea.
       rewrite rename_closed. 2: assumption.
-      eapply (PCUICClosed.declared_constant_closed_body). all: eauto.
+      eapply (PCUICClosedTyping.declared_constant_closed_body). all: eauto.
     - rewrite rename_mkApps. simpl. cbn in H0; inv_on_free_vars.
       econstructor; tea. 2:erewrite nth_error_map, heq_nth_error; reflexivity.
       solve_all.
@@ -2309,7 +2309,7 @@ Section ParallelSubstitution.
 
     - simpl. rewrite inst_closed0.
       rewrite PCUICClosed.closedn_subst_instance; auto.
-      eapply (PCUICClosed.declared_constant_closed_body). all: eauto.
+      eapply (PCUICClosedTyping.declared_constant_closed_body). all: eauto.
       econstructor; eauto with pcuic.
 
     - eapply pred1_refl_gen. now apply pred1_subst_pred1_ctx in Hrel.
