pcuic/theories/PCUICReduction.v
@@ -2,7 +2,7 @@
 From MetaCoq.Template Require Import config utils.
 From MetaCoq.PCUIC Require Import PCUICAst PCUICAstUtils
      PCUICLiftSubst PCUICUnivSubst PCUICInduction 
-     PCUICContextRelation PCUICCases.
+     PCUICContextRelation PCUICCases PCUICOnFreeVars PCUICClosed PCUICTyping.
 
 Require Import ssreflect.
 Require Import Equations.Prop.DepElim.
@@ -25,7 +25,7 @@ Proof.
     + constructor. eassumption.
     + clear - IHh. rename IHh into h.
       induction h.
-      * constructor.
+      * constructor. 
       * econstructor.
         -- econstructor 2. eassumption.
         -- assumption.
@@ -35,22 +35,6 @@ Definition tDummy := tVar String.EmptyString.
 Definition dummy_branch : branch term := mk_branch [] tDummy.
 
 (** ** Reduction *)
-
-Lemma fix_subst_length mfix : #|fix_subst mfix| = #|mfix|.
-Proof.
-  unfold fix_subst. generalize (tFix mfix). intros.
-  induction mfix; simpl; auto.
-Qed.
-
-Lemma cofix_subst_length mfix : #|cofix_subst mfix| = #|mfix|.
-Proof.
-  unfold cofix_subst. generalize (tCoFix mfix). intros.
-  induction mfix; simpl; auto.
-Qed.
-
-Lemma fix_context_length mfix : #|fix_context mfix| = #|mfix|.
-Proof. unfold fix_context. now rewrite List.rev_length mapi_length. Qed.
-
 
 (** *** One step strong beta-zeta-iota-fix-delta reduction
 
@@ -1471,8 +1455,6 @@ Section ReductionCongruence.
           { now destruct p. }
           eapply red_one_param; eassumption.
     Qed.
-
-    Coercion ci_ind : case_info >-> inductive.
     
     (* Lemma red_one_pcontext :
       forall ci p c brs pcontext',
@@ -1594,7 +1576,10 @@ Section ReductionCongruence.
 
     Lemma All3_length {A B C} {R : A -> B -> C -> Type} l l' l'' :
       All3 R l l' l'' -> #|l| = #|l'| /\ #|l'| = #|l''|.
-    Proof. induction 1; simpl; intuition auto. Qed.
+    Proof. induction 1; simpl; intuition auto.
+           - f_equal. assumption.
+           - f_equal. assumption.  
+    Qed.
 
     Lemma All3_many_OnOne2All :
       forall B A (R : B -> A -> A -> Type) lΔ l l',
@@ -2427,123 +2412,5 @@ Section Stacks.
 
 End Stacks.
 
-(** Not used anywhere *)
-(*
-(* Properties about context closure *)
-(** Reductions at top level *)
-Inductive tred1 (Σ : global_env) (Γ : context) : term -> term -> Type :=
+Implicit Types (cf : checker_flags).
 
-(** Beta *)
-| tred_beta na t b a :
-    tred1 Σ Γ (tApp (tLambda na t b) a) (subst10 a b)
-
-(** Let *)
-| tred_zeta na b t b' :
-    tred1 Σ Γ (tLetIn na b t b') (subst10 b b')
-
-| tred_rel i body :
-    option_map decl_body (nth_error Γ i) = Some (Some body) ->
-    tred1 Σ Γ (tRel i) (lift0 (S i) body)
-
-(** Case *)
-| tred_iota ci c u args p brs :
-    tred1 Σ Γ (tCase ci p (mkApps (tConstruct ci.(ci_ind) c u) args) brs)
-         (iota_red ci.(ci_npar) c args brs)
-
-(** Fix unfolding, with guard *)
-| tred_fix mfix idx args narg fn :
-    unfold_fix mfix idx = Some (narg, fn) ->
-    is_constructor narg args = true ->
-    tred1 Σ Γ (mkApps (tFix mfix idx) args) (mkApps fn args)
-
-(** CoFix-case unfolding *)
-| tred_cofix_case ip p mfix idx args narg fn brs :
-    unfold_cofix mfix idx = Some (narg, fn) ->
-    tred1 Σ Γ (tCase ip p (mkApps (tCoFix mfix idx) args) brs)
-         (tCase ip p (mkApps fn args) brs)
-
-(** CoFix-proj unfolding *)
-| tred_cofix_proj p mfix idx args narg fn :
-    unfold_cofix mfix idx = Some (narg, fn) ->
-    tred1 Σ Γ (tProj p (mkApps (tCoFix mfix idx) args))
-         (tProj p (mkApps fn args))
-
-(** Constant unfolding *)
-| tred_delta c decl body (isdecl : declared_constant Σ c decl) u :
-    decl.(cst_body) = Some body ->
-    tred1 Σ Γ (tConst c u) (subst_instance u body)
-
-(** Proj *)
-| tred_proj i pars narg args u arg:
-    nth_error args (pars + narg) = Some arg ->
-    tred1 Σ Γ (tProj (i, pars, narg) (mkApps (tConstruct i 0 u) args)) arg.
-
-Definition ctred1 Σ :=
-  context_env_clos (tred1 Σ).
-
-(* TODO Prove context_clos_impl using subrelation *)
-
-Lemma tred1_red1 :
-  forall Σ Γ u v,
-    tred1 Σ Γ u v ->
-    red1 Σ Γ u v.
-Proof.
-  intros Σ Γ u v h.
-  destruct h.
-  all: solve [
-    econstructor ; eauto
-  ].
-Qed.
-
-Lemma ctred1_red1 :
-  forall Σ Γ u v,
-    ctred1 Σ Γ u v ->
-    red1 Σ Γ u v.
-Proof.
-  intros Σ Γ u' v' [u [v [π [h [? ?]]]]]. subst.
-  induction π in Γ, u, v, h |- * using stack_rev_rect.
-  all: try solve [
-    rewrite 2!zipc_stack_cat ; cbn ;
-    rewrite stack_context_stack_cat in h ; cbn in h ;
-    rewrite ?app_context_nil_l ?app_context_assoc in h ;
-    econstructor ; eapply IHπ ; eassumption
-  ].
-  - cbn. eapply tred1_red1. assumption.
-  - rewrite 2!zipc_stack_cat. cbn.
-    rewrite stack_context_stack_cat in h. cbn in h.
-    rewrite app_context_nil_l in h.
-    eapply fix_red_ty. eapply OnOne2_app. constructor. cbn.
-    intuition auto.
-  - rewrite 2!zipc_stack_cat. cbn.
-    rewrite stack_context_stack_cat in h. cbn in h.
-    rewrite app_context_nil_l in h.
-    eapply fix_red_body. eapply OnOne2_app. constructor. cbn.
-    intuition auto.
-    eapply IHπ.
-    rewrite fix_context_fix_context_alt.
-    rewrite map_app. cbn. unfold def_sig at 2. cbn.
-    rewrite app_context_assoc in h.
-    assumption.
-  - rewrite 2!zipc_stack_cat. cbn.
-    rewrite stack_context_stack_cat in h. cbn in h.
-    rewrite app_context_nil_l in h.
-    eapply cofix_red_ty. eapply OnOne2_app. constructor. cbn.
-    intuition auto.
-  - rewrite 2!zipc_stack_cat. cbn.
-    rewrite stack_context_stack_cat in h. cbn in h.
-    rewrite app_context_nil_l in h.
-    eapply cofix_red_body. eapply OnOne2_app. constructor. cbn.
-    intuition auto.
-    eapply IHπ.
-    rewrite fix_context_fix_context_alt.
-    rewrite map_app. cbn. unfold def_sig at 2. cbn.
-    rewrite app_context_assoc in h.
-    assumption.
-  - rewrite 2!zipc_stack_cat. cbn.
-    rewrite stack_context_stack_cat in h. cbn in h.
-    rewrite app_context_nil_l in h.
-    econstructor. eapply OnOne2_app. constructor. cbn.
-    intuition auto.
-  -
-Qed.
-*)
