pcuic/theories/Typing/PCUICInstTyp.v
@@ -1,0 +1,265 @@
+(* Distributed under the terms of the MIT license. *)
+From Coq Require Import Morphisms.
+From MetaCoq.Template Require Import config utils.
+From MetaCoq.PCUIC Require Import PCUICAst PCUICAstUtils PCUICCases PCUICInduction
+  PCUICLiftSubst PCUICUnivSubst PCUICContextRelation
+  PCUICTyping PCUICReduction PCUICCumulativity 
+  PCUICEquality PCUICGlobalEnv PCUICClosed PCUICClosedTyping PCUICEquality PCUICWeakeningEnvConv PCUICWeakeningEnvTyp
+  PCUICSigmaCalculus PCUICRenameDef PCUICRenameConv PCUICWeakening PCUICInstDef PCUICInstConv
+  PCUICGuardCondition PCUICUnivSubstitutionConv PCUICOnFreeVars.
+
+Require Import ssreflect ssrbool.
+From Equations Require Import Equations.
+Require Import Equations.Prop.DepElim.
+Set Equations With UIP.
+Set Keyed Unification.
+Set Default Goal Selector "!".
+Implicit Types cf : checker_flags.
+
+(** * Type preservation for σ-calculus instantiation *)
+
+Open Scope sigma_scope.
+
+Lemma inst_cumulSpec {cf : checker_flags} {Σ : global_env_ext} {wfΣ : wf Σ} {P Γ Δ σ A B} :
+  usubst Γ σ Δ ->
+  on_free_vars P A ->
+  on_free_vars P B ->
+  on_ctx_free_vars P Γ ->
+  Σ ;;; Γ |- A <=s B ->
+  Σ ;;; Δ |- A.[σ] <=s B.[σ].
+Admitted. 
+
+Lemma type_inst {cf : checker_flags} : env_prop
+  (fun Σ Γ t A =>
+    forall Δ σ,
+    wf_local Σ Δ ->
+    Σ ;;; Δ ⊢ σ : Γ ->
+    Σ ;;; Δ |- t.[σ] : A.[σ])
+  (fun Σ Γ =>
+    All_local_env
+    (lift_typing (fun (Σ : global_env_ext) (Γ : context) (t T : term)
+    =>
+    forall Δ σ,
+    wf_local Σ Δ ->
+    Σ ;;; Δ ⊢ σ : Γ ->
+    Σ ;;; Δ |- t.[σ] : T.[σ]) Σ) Γ).
+Proof.
+  apply typing_ind_env.
+
+  - intros Σ wfΣ Γ wfΓ. auto.
+    induction 1; constructor; firstorder auto.
+  - intros Σ wfΣ Γ wfΓ n decl e X Δ σ hΔ hσ. simpl.
+    eapply hσ. assumption.
+  - intros Σ wfΣ Γ wfΓ l X H0 Δ σ hΔ hσ. simpl.
+    econstructor. all: assumption.
+  - intros Σ wfΣ Γ wfΓ na A B s1 s2 X hA ihA hB ihB Δ σ hΔ hσ.
+    autorewrite with sigma. simpl.
+    econstructor.
+    + eapply ihA ; auto.
+    + eapply ihB.
+      * econstructor ; auto.
+        eexists. eapply ihA ; auto.
+      * eapply well_subst_Up. 2: assumption.
+        econstructor ; auto.
+        eexists. eapply ihA. all: auto.
+  - intros Σ wfΣ Γ wfΓ na A t s1 bty X hA ihA ht iht Δ σ hΔ hσ.
+    autorewrite with sigma.
+    econstructor.
+    + eapply ihA ; auto.
+    + eapply iht.
+      * econstructor ; auto.
+        eexists. eapply ihA ; auto.
+      * eapply well_subst_Up. 2: assumption.
+        constructor. 1: assumption.
+        eexists. eapply ihA. all: auto.
+  - intros Σ wfΣ Γ wfΓ na b B t s1 A X hB ihB hb ihb ht iht Δ σ hΔ hσ.
+    autorewrite with sigma.
+    econstructor.
+    + eapply ihB. all: auto.
+    + eapply ihb. all: auto.
+    + eapply iht.
+      * econstructor. all: auto.
+        -- eexists. eapply ihB. all: auto.
+        -- simpl. eapply ihb. all: auto.
+      * eapply well_subst_Up'; try assumption.
+        constructor; auto.
+        ** exists s1. apply ihB; auto.
+        ** apply ihb; auto.
+  - intros Σ wfΣ Γ wfΓ t na A B s u X hty ihty ht iht hu ihu Δ σ hΔ hσ.
+    autorewrite with sigma.
+    econstructor.
+    * specialize (ihty _ _ hΔ hσ).
+      simpl in ihty. eapply meta_conv_term; [eapply ihty|].
+      now rewrite up_Up.
+    * specialize (iht _ _ hΔ hσ).
+      simpl in iht. eapply meta_conv; [eapply iht|].
+      now rewrite up_Up.
+    * eapply ihu; auto.
+  - intros Σ wfΣ Γ wfΓ cst u decl X X0 isdecl hconst Δ σ hΔ hσ.
+    autorewrite with sigma. simpl.
+    eapply meta_conv; [econstructor; eauto|].
+    eapply declared_constant_closed_type in isdecl; eauto.
+    rewrite inst_closed0; auto.
+    now rewrite closedn_subst_instance.
+  - intros Σ wfΣ Γ wfΓ ind u mdecl idecl isdecl X X0 hconst Δ σ hΔ hσ.
+    eapply meta_conv; [econstructor; eauto|].
+    eapply declared_inductive_closed_type in isdecl; eauto.
+    rewrite inst_closed0; auto.
+    now rewrite closedn_subst_instance.
+  - intros Σ wfΣ Γ wfΓ ind i u mdecl idecl cdecl isdecl X X0 hconst Δ σ hΔ hσ.
+    eapply meta_conv; [econstructor; eauto|].
+    eapply declared_constructor_closed_type in isdecl; eauto.
+    rewrite inst_closed0; eauto.
+  - intros Σ wfΣ Γ wfΓ ci p c brs indices ps mdecl idecl isdecl HΣ.
+    intros IHΔ ci_npar eqpctx predctx wfp cup Hpctx Hpret
+      IHpret IHpredctx isallowed.
+    intros Hctxi IHctxi Hc IHc iscof ptm wfbrs Hbrs Δ f HΔ Hf.
+    autorewrite with sigma. simpl.
+    rewrite map_app. simpl.
+    rewrite /ptm. rewrite inst_it_mkLambda_or_LetIn.
+    relativize #|predctx|.
+    * erewrite inst_predicate_preturn.
+      rewrite /predctx.
+      rewrite inst_case_predicate_context //.
+      eapply type_Case; eauto;
+       rewrite - ?inst_case_predicate_context //.
+      + now eapply inst_wf_predicate.
+      + simpl.
+        apply All_local_env_app_inv in Hpctx as [].
+        eapply wf_local_app_inst; eauto.
+        apply All_local_env_app_inv in IHpredctx as [].
+        apply a2.
+      + apply All_local_env_app_inv in Hpctx as [].
+        apply All_local_env_app_inv in IHpredctx as [].
+        eapply IHpret.
+        ++ eapply wf_local_app_inst; eauto.
+           apply a2.
+        ++ relativize #|pcontext p|; [eapply well_subst_app_up|] => //; rewrite /predctx; len.
+           2:{ rewrite case_predicate_context_length //. }
+           eapply wf_local_app_inst; eauto. apply a2.
+      + revert IHctxi.
+        rewrite /= /id -map_app.
+        rewrite -{2}[subst_instance _ _](inst_closedn_ctx f 0).
+        { pose proof (declared_inductive_closed_pars_indices isdecl).
+          now rewrite closedn_subst_instance_context. }
+        rewrite inst_context_telescope.
+        rewrite inst_telescope_upn0.
+        clear -Δ f HΔ Hf.
+        induction 1.
+        { constructor; auto. }
+        { simpl. rewrite inst_telescope_cons.
+          constructor; cbn; eauto.
+          now rewrite inst_subst_telescope /= in IHIHctxi. }
+        { simpl. rewrite inst_telescope_cons.
+          constructor; cbn; eauto.
+          now rewrite inst_subst_telescope /= in IHIHctxi. }
+      + simpl. unfold id.
+        specialize (IHc _ _ HΔ Hf).
+        now rewrite inst_mkApps map_app in IHc.
+      + now eapply inst_wf_branches.
+      + eapply Forall2_All2 in wfbrs.
+        eapply All2i_All2_mix_left in Hbrs; eauto.
+        eapply All2i_nth_hyp in Hbrs.
+        eapply All2i_map_right, (All2i_impl Hbrs) => i cdecl br.
+        set (brctxty := case_branch_type _ _ _ _ _ _ _ _).
+        move=> [Hnth [wfbr [Hconv [Hbrctx [Hbr [IHbr [Hbty IHbty]]]]]]].
+        split => //.
+        rewrite -(inst_closed_constructor_body mdecl cdecl f).
+        { eapply (declared_constructor_closed (c:=(ci.(ci_ind),i))); eauto.
+          split; eauto. }
+        rewrite inst_case_predicate_context //.
+        rewrite inst_case_branch_type //.
+        rewrite -/brctxty. intros brctx'.
+        assert (wf_local Σ (Δ,,, brctx'.1)).
+        { rewrite /brctx'. cbn.
+          apply All_local_env_app_inv in Hbrctx as [].
+          eapply wf_local_app_inst; tea. apply a0. }
+        split => //. split.
+        ++ eapply IHbr => //.
+          rewrite /brctx' /brctxty; cbn.
+          relativize #|bcontext br|.
+          { eapply well_subst_app_up => //. }
+          rewrite /case_branch_type /=.
+          rewrite case_branch_context_length //.
+        ++ eapply IHbty=> //.
+          rewrite /brctx'; cbn.
+          relativize #|bcontext br|.
+          { eapply well_subst_app_up => //. }
+          rewrite /brctxty /= case_branch_context_length //.
+    * rewrite /predctx case_predicate_context_length //.
+  - intros Σ wfΣ Γ wfΓ p c u mdecl idecl cdecl pdecl isdecl args X X0 hc ihc e ty
+           Δ σ hΔ hσ.
+    simpl.
+    eapply meta_conv; [econstructor|].
+    * eauto.
+    * specialize (ihc _ _ hΔ hσ).
+      rewrite inst_mkApps in ihc. eapply ihc.
+    * now rewrite map_length.
+    * autorewrite with sigma.
+      eapply declared_projection_closed in isdecl; auto.
+      move: isdecl.
+      rewrite -(closedn_subst_instance _ _ u).
+      rewrite /ty.
+      eapply inst_ext_closed.
+      intros x Hx.
+      rewrite subst_consn_lt /=; len; try lia.
+      (rewrite Upn_comp; try now repeat len); [].
+      rewrite subst_consn_lt /=; len; try lia.
+      now rewrite map_rev.
+  - intros Σ wfΣ Γ wfΓ mfix n decl types hguard hnth htypes hmfix ihmfix wffix Δ σ hΔ hσ.
+    simpl. eapply meta_conv; [econstructor;eauto|].
+    * now eapply fix_guard_inst.
+    * now rewrite nth_error_map hnth.
+    * solve_all.
+      destruct a as [s [Hs IH]].
+      exists s; eapply IH; eauto.
+    * solve_all.
+      len. rewrite /types in b0. len in b0.
+      pose proof (inst_fix_context mfix σ).
+      setoid_rewrite <-up_Upn at 1 in H. rewrite H.
+      eapply All_local_env_app_inv in htypes as [].
+      eapply meta_conv; [eapply b0; eauto|].
+      + eapply wf_local_app_inst; eauto. eapply a2.
+      + rewrite -(fix_context_length mfix).
+        eapply well_subst_app_up => //.
+        eapply wf_local_app_inst; eauto. apply a2.
+      + rewrite lift0_inst. now sigma.
+    * now apply inst_wf_fixpoint.
+    * reflexivity.
+
+  - intros Σ wfΣ Γ wfΓ mfix n decl types hguard hnth htypes hmfix ihmfix wffix Δ σ hΔ hσ.
+    simpl. eapply meta_conv; [econstructor;eauto|].
+    * now eapply cofix_guard_inst.
+    * now rewrite nth_error_map hnth.
+    * solve_all.
+      destruct a as [s [Hs IH]].
+      exists s; eapply IH; eauto.
+    * solve_all.
+      len. rewrite /types in b0. len in b0.
+      pose proof (inst_fix_context mfix σ).
+      setoid_rewrite <-up_Upn at 1 in H. rewrite H.
+      eapply All_local_env_app_inv in htypes as [].
+      eapply meta_conv; [eapply b0; eauto|].
+      + eapply wf_local_app_inst; eauto. eapply a2.
+      + rewrite -(fix_context_length mfix).
+        eapply well_subst_app_up => //.
+        eapply wf_local_app_inst; eauto. apply a2.
+      + rewrite lift0_inst. now sigma.
+    * now apply inst_wf_cofixpoint.
+    * reflexivity.
+
+  - intros Σ wfΣ Γ wfΓ t A B X hwf ht iht hB ihB hcum Δ σ hΔ hσ.
+    eapply type_Cumul.
+    + eapply iht. all: auto.
+    + eapply ihB. all: auto.
+    + eapply inst_cumulSpec => //.
+      * exact hσ.
+      * eapply type_closed in ht.
+        now eapply closedn_on_free_vars.
+      * eapply subject_closed in hB.
+        now eapply closedn_on_free_vars.
+      * eapply closed_wf_local in wfΓ; tea.
+        rewrite closedn_ctx_on_free_vars in wfΓ.
+        now rewrite -on_free_vars_ctx_on_ctx_free_vars in wfΓ.
+      * apply hcum.
+Qed.
