pcuic/theories/Typing/PCUICRenameTyp.v
@@ -1,0 +1,820 @@
+(* Distributed under the terms of the MIT license. *)
+From Coq Require Import Morphisms.
+From MetaCoq.Template Require Import config utils.
+From MetaCoq.PCUIC Require Import PCUICAst PCUICAstUtils PCUICCases PCUICInduction
+  PCUICLiftSubst PCUICUnivSubst PCUICContextRelation PCUICCumulativity
+  PCUICTyping PCUICReduction PCUICGlobalEnv PCUICClosed PCUICEquality PCUICRenameDef 
+  PCUICSigmaCalculus PCUICClosed PCUICOnFreeVars PCUICGuardCondition PCUICTyping
+  PCUICWeakeningEnvConv PCUICWeakeningEnvTyp PCUICClosedTyping PCUICRenameConv.
+
+Require Import ssreflect ssrbool.
+From Equations Require Import Equations.
+Require Import Equations.Prop.DepElim.
+Set Equations With UIP.
+
+(** * Type preservation for σ-calculus operations *)
+
+Open Scope sigma_scope.
+Set Keyed Unification.
+
+Set Default Goal Selector "!".
+
+
+Section Renaming.
+
+Context `{cf : checker_flags}.
+
+Lemma renaming_vass :
+  forall P Σ Γ Δ na A f,
+    wf_local Σ (Γ ,, vass na (rename f A)) ->
+    renaming P Σ Γ Δ f ->
+    renaming (shiftnP 1 P) Σ (Γ ,, vass na (rename f A)) (Δ ,, vass na A) (shiftn 1 f).
+Proof.
+  intros P Σ Γ Δ na A f hΓ [? h].
+  split. 1: auto.
+  eapply urenaming_vass; assumption.
+Qed.
+
+Lemma renaming_vdef :
+  forall P Σ Γ Δ na b B f,
+    wf_local Σ (Γ ,, vdef na (rename f b) (rename f B)) ->
+    renaming P Σ Γ Δ f ->
+    renaming (shiftnP 1 P) Σ (Γ ,, vdef na (rename f b) (rename f B)) (Δ ,, vdef na b B) (shiftn 1 f).
+Proof.
+  intros P Σ Γ Δ na b B f hΓ [? h].
+  split. 1: auto.
+  eapply urenaming_vdef; assumption.
+Qed.
+
+Lemma rename_ind_predicate_context {Σ : global_env_ext} {wfΣ : wf Σ} {f ind mdecl idecl} :
+  declared_inductive Σ ind mdecl idecl ->
+  rename_context (shiftn (context_assumptions (ind_params mdecl)) f) (ind_predicate_context ind mdecl idecl) =
+  ind_predicate_context ind mdecl idecl.
+Proof.
+  intros isdecl.
+  generalize (declared_inductive_closed_pars_indices isdecl).
+  rewrite closedn_ctx_app => /andP [] clpars /= clinds.
+  rewrite /ind_predicate_context.
+  rewrite /expand_lets_ctx /expand_lets_k_ctx.
+  rewrite !rename_context_snoc /= /map_decl /= /snoc. f_equal.
+  - f_equal. len.
+    rewrite rename_mkApps /=. f_equal.
+    rewrite shiftn_add.
+    relativize (#|_| + _).
+    1:now erewrite -> rename_to_extended_list.
+    now len.
+  - rewrite rename_context_subst.
+    rewrite rename_closed_extended_subst //. f_equal.
+    rewrite shiftn_add Nat.add_comm. len.
+    rewrite rename_context_lift. f_equal. 
+    rewrite rename_closedn_ctx //.
+Qed.
+
+Lemma rename_case_predicate_context {Σ : global_env_ext} {wfΣ : wf Σ} {ind mdecl idecl f p} :
+  declared_inductive Σ ind mdecl idecl ->
+  wf_predicate mdecl idecl p ->
+  rename_context f (case_predicate_context ind mdecl idecl p) =
+  case_predicate_context ind mdecl idecl (rename_predicate f p).
+Proof.
+  intros decli wfp.
+  unfold case_predicate_context. simpl.
+  unfold id. unfold case_predicate_context_gen.
+  rewrite rename_context_set_binder_name.
+  - len.
+    now rewrite -(wf_predicate_length_pcontext wfp).
+  - f_equal. rewrite /pre_case_predicate_context_gen.
+    rewrite rename_inst_case_context.
+    rewrite (wf_predicate_length_pars wfp) (declared_minductive_ind_npars decli).
+    now rewrite (rename_ind_predicate_context decli).
+Qed.
+
+Lemma rename_case_branch_type {Σ : global_env_ext} {wfΣ : wf Σ} f (ci : case_info) mdecl idecl p br i cdecl :
+  declared_inductive Σ ci mdecl idecl ->
+  wf_predicate mdecl idecl p ->
+  wf_branch cdecl br ->
+  let ptm := it_mkLambda_or_LetIn (case_predicate_context ci mdecl idecl p) (preturn p) in
+  let p' := rename_predicate f p in
+  let ptm' := it_mkLambda_or_LetIn (case_predicate_context ci mdecl idecl p') (preturn p') in
+  case_branch_type ci mdecl idecl
+     (rename_predicate f p)
+     (map_branch_shift rename shiftn f br)
+     ptm' i (rename_constructor_body mdecl f cdecl) =
+  map_pair (rename_context f) (rename (shiftn #|bcontext br| f))
+  (case_branch_type ci mdecl idecl p br ptm i cdecl).
+Proof.
+  intros decli wfp wfb ptm p' ptm'.
+  rewrite /case_branch_type /case_branch_type_gen /map_pair /=.
+  rewrite rename_case_branch_context_gen //.
+  { eapply (declared_inductive_closed_params decli). }
+  { len; now apply wf_branch_length. }
+  { rewrite -(declared_minductive_ind_npars decli).
+    apply (wf_predicate_length_pars wfp). }
+  f_equal.
+  rewrite rename_mkApps map_app map_map_compose.
+  rewrite (wf_branch_length wfb).
+  f_equal.
+  * rewrite /ptm' /ptm !lift_it_mkLambda_or_LetIn !rename_it_mkLambda_or_LetIn.
+    rewrite !lift_rename. f_equal.
+    ++ rewrite /p'. len.
+      epose proof (rename_context_lift f #|cstr_args cdecl| 0).
+        rewrite Nat.add_0_r in H.
+        rewrite H. len.
+        rewrite shiftn0 //. f_equal.
+        rewrite rename_case_predicate_context //.
+    ++ rewrite /p'. rewrite Nat.add_0_r. simpl. len.
+      rewrite map2_length //. 1:{ len. now rewrite (wf_predicate_length_pcontext wfp). }
+      rewrite - !lift_rename; len. rewrite case_predicate_context_length // shiftn_add.
+      now rewrite -rename_shiftnk Nat.add_comm.
+  * rewrite /= rename_mkApps /=. f_equal.
+    ++ rewrite !map_map_compose /id. apply map_ext => t.
+      rewrite /expand_lets /expand_lets_k.
+      rewrite -rename_subst_instance. len.
+      rewrite -shiftn_add -shiftn_add.
+      rewrite rename_subst map_rev. f_equal.
+      rewrite List.rev_length rename_subst.
+      rewrite (wf_predicate_length_pars wfp).
+      rewrite (declared_minductive_ind_npars decli).
+      rewrite -{2}(context_assumptions_subst_instance (puinst p) (ind_params mdecl)).
+      rewrite rename_closed_extended_subst.
+      { rewrite closedn_subst_instance_context.
+        apply (declared_inductive_closed_params decli). }
+      f_equal. len. rewrite !shiftn_add.
+      rewrite (Nat.add_comm _ (context_assumptions _)) rename_shiftnk.
+      f_equal. rewrite Nat.add_comm rename_subst.
+      rewrite rename_inds. f_equal.
+      rewrite shiftn_add. len. lia_f_equal.
+    ++ unfold id. f_equal. f_equal.
+       rewrite map_app map_map_compose.
+       rewrite map_map_compose.
+       setoid_rewrite rename_shiftn. len. f_equal.
+       rewrite rename_to_extended_list.
+       now rewrite /to_extended_list /to_extended_list_k reln_fold.
+Qed.
+
+
+
+Lemma convSpec_renameP :
+  forall P Σ Γ Δ f A B,
+    wf Σ.1 ->
+    urenaming P Δ Γ f ->
+    on_free_vars P A ->
+    on_free_vars P B ->
+    on_ctx_free_vars P Γ ->
+    Σ ;;; Γ |- A =s B ->
+    Σ ;;; Δ |- rename f A =s rename f B.
+Admitted. 
+
+Lemma cumulSpec_renameP :
+  forall P Σ Γ Δ f A B,
+    wf Σ.1 ->
+    urenaming P Δ Γ f ->
+    on_free_vars P A ->
+    on_free_vars P B ->
+    on_ctx_free_vars P Γ ->
+    Σ ;;; Γ |- A <=s B ->
+    Σ ;;; Δ |- rename f A <=s rename f B.
+Admitted.
+
+Lemma cumul_decls_renameP {P Σ Γ Γ' Δ Δ' f} d d' :
+    wf Σ.1 ->
+    urenaming P Δ Γ f ->
+    urenaming P Δ' Γ' f ->
+    on_free_vars_decl P d ->
+    on_free_vars_decl P d' ->
+    on_ctx_free_vars P Γ ->
+    cumul_decls Σ Γ Γ' d d' ->
+    cumul_decls Σ Δ Δ' (rename_decl f d) (rename_decl f d').
+Proof.
+  intros wf uren uren' ond ond' onΓ Hd; depelim Hd; constructor; tas;
+    (eapply convSpec_renameP || eapply cumulSpec_renameP); tea.
+  * now move/andP: ond => [].
+  * now move/andP: ond' => [].
+  * now move/andP: ond => [].
+  * now move/andP: ond' => [].
+Qed.
+
+Lemma conv_decls_renameP {P Σ Γ Γ' Δ Δ' f} d d' :
+    wf Σ.1 ->
+    urenaming P Δ Γ f ->
+    urenaming P Δ' Γ' f ->
+    on_free_vars_decl P d ->
+    on_free_vars_decl P d' ->
+    on_ctx_free_vars P Γ ->
+    conv_decls Σ Γ Γ' d d' ->
+    conv_decls Σ Δ Δ' (rename_decl f d) (rename_decl f d').
+Proof.
+  intros wf uren uren' ond ond' onΓ Hd; depelim Hd; constructor; tas;
+    (eapply convSpec_renameP || eapply cumulSpec_renameP); tea.
+  * now move/andP: ond => [].
+  * now move/andP: ond' => [].
+  * now move/andP: ond => [].
+  * now move/andP: ond' => [].
+Qed.
+
+Lemma on_free_vars_ctx_onctx_k P ctx :
+  reflectT (onctx_k (fun k => on_free_vars (shiftnP k P)) 0 ctx)
+    (on_free_vars_ctx P ctx).
+Proof.
+  rewrite -test_context_k_on_free_vars_ctx.
+  apply (onctx_k_P reflectT_pred2).
+Qed.
+
+Lemma Alli_helper Q Γ :
+  Alli (fun (i : nat) (d : context_decl) => ondecl (Q (#|Γ| - i + 0)) d) 1 Γ ->
+  onctx_k Q 0 Γ.
+Proof.
+  move/(Alli_shiftn_inv 0 _ 1) => H.
+  eapply Alli_impl; tea => n x /=.
+  now replace (#|Γ| - S n + 0) with (Nat.pred #|Γ| - n + 0) by lia.
+Qed.
+
+Lemma All2_fold_impl_ind_onctx_k Q P P' Γ Δ :
+  onctx_k Q 0 Γ ->
+  onctx_k Q 0 Δ ->
+  All2_fold P Γ Δ ->
+  (forall Γ Δ d d',
+    All2_fold P Γ Δ ->
+    onctx_k Q 0 Γ ->
+    All2_fold P' Γ Δ ->
+    ondecl (Q #|Γ|) d ->
+    ondecl (Q #|Δ|) d' ->
+    P Γ Δ d d' ->
+    P' Γ Δ d d') ->
+  All2_fold P' Γ Δ.
+Proof.
+  intros qΓ qΔ cr Hcr.
+  induction cr in qΓ, qΔ |- *; constructor; depelim qΓ; depelim qΔ; intuition eauto;
+  rewrite -> Nat.sub_0_r, Nat.add_0_r in *;
+  apply Alli_helper in qΓ; apply Alli_helper in qΔ;
+  simpl in *; eauto.
+Qed.
+
+Lemma ondecl_on_free_vars_decl P d :
+  ondecl (on_free_vars P) d ->
+  on_free_vars_decl P d.
+Proof.
+  rewrite /on_free_vars_decl.
+  now case: (ondeclP reflectT_pred).
+Qed.
+
+Lemma conv_ctx_renameP {Σ : global_env_ext} {P} {Γ Δ} {L R} f :
+  wf Σ.1 ->
+  urenaming P Δ Γ f ->
+  on_free_vars_ctx P L ->
+  on_free_vars_ctx P R ->
+  on_ctx_free_vars P Γ ->
+  conv_context Σ (Γ ,,, L) (Γ ,,, R) ->
+  conv_context Σ (Δ ,,, rename_context f L) (Δ ,,, rename_context f R).
+Proof.
+  intros wf uren onL onL' onΓ H.
+  rewrite /rename_context - !mapi_context_fold.
+  pose proof (All2_fold_length H) as hlen.
+  len in hlen. assert (#|L| = #|R|) by lia.
+  eapply All2_fold_app_inv in H as [_ H] => //.
+  eapply All2_fold_app; len => //; pcuic.
+  { eapply conv_ctx_refl'. }
+  move/on_free_vars_ctx_onctx_k: onL => onL.
+  move/on_free_vars_ctx_onctx_k: onL' => onR.
+
+  eapply All2_fold_mapi.
+  eapply All2_fold_impl_ind_onctx_k; tea =>
+    /= L' R' d d' IH onL' IH' ond ond'.
+  simpl.
+  rewrite !mapi_context_fold -/(rename_context f L') -/(rename_context f R').
+  eapply conv_decls_renameP; eauto.
+  + now eapply urenaming_context.
+  + rewrite (All2_fold_length IH).
+    now eapply urenaming_context.
+  + now eapply ondecl_on_free_vars_decl.
+  + rewrite (All2_fold_length IH').
+    now eapply ondecl_on_free_vars_decl.
+  + rewrite on_ctx_free_vars_extend // onΓ.
+    now move/on_free_vars_ctx_onctx_k: onL'.
+Qed.
+
+Lemma cumul_ctx_renameP {Σ : global_env_ext} {P} {Γ Δ} {L R} f :
+  wf Σ.1 ->
+  urenaming P Δ Γ f ->
+  on_free_vars_ctx P L ->
+  on_free_vars_ctx P R ->
+  on_ctx_free_vars P Γ ->
+  cumul_context Σ (Γ ,,, L) (Γ ,,, R) ->
+  cumul_context Σ (Δ ,,, rename_context f L) (Δ ,,, rename_context f R).
+Proof.
+  intros wf uren onL onL' onΓ H.
+  rewrite /rename_context - !mapi_context_fold.
+  pose proof (All2_fold_length H) as hlen.
+  len in hlen. assert (#|L| = #|R|) by lia.
+  eapply All2_fold_app_inv in H as [_ H] => //.
+  eapply All2_fold_app; len => //; pcuic.
+  { eapply cumul_ctx_refl'. }
+  move/on_free_vars_ctx_onctx_k: onL => onL.
+  move/on_free_vars_ctx_onctx_k: onL' => onR.
+
+  eapply All2_fold_mapi.
+  eapply All2_fold_impl_ind_onctx_k; tea =>
+    /= L' R' d d' IH onL' IH' ond ond'.
+  simpl.
+  rewrite !mapi_context_fold -/(rename_context f L') -/(rename_context f R').
+  eapply cumul_decls_renameP; eauto.
+  + now eapply urenaming_context.
+  + rewrite (All2_fold_length IH).
+    now eapply urenaming_context.
+  + now eapply ondecl_on_free_vars_decl.
+  + rewrite (All2_fold_length IH').
+    now eapply ondecl_on_free_vars_decl.
+  + rewrite on_ctx_free_vars_extend // onΓ.
+    now move/on_free_vars_ctx_onctx_k: onL'.
+Qed.
+
+Lemma subst1_inst :
+  forall t n u,
+    t{ n := u } = t.[⇑^n (u ⋅ ids)].
+Proof.
+  intros t n u.
+  unfold subst1. rewrite subst_inst.
+  eapply inst_ext. intro i.
+  unfold Upn, subst_compose, subst_consn.
+  destruct (Nat.ltb_spec0 i n).
+  - rewrite -> nth_error_idsn_Some by assumption. reflexivity.
+  - rewrite -> nth_error_idsn_None by lia.
+    rewrite idsn_length.
+    destruct (Nat.eqb_spec (i - n) 0).
+    + rewrite e. simpl. reflexivity.
+    + replace (i - n) with (S (i - n - 1)) by lia. simpl.
+      destruct (i - n - 1) eqn: e.
+      * simpl. reflexivity.
+      * simpl. reflexivity.
+Qed.
+(* Hint Rewrite @subst1_inst : sigma. *)
+
+Lemma rename_predicate_preturn f p :
+  rename (shiftn #|p.(pcontext)| f) (preturn p) =
+  preturn (rename_predicate f p).
+Proof. reflexivity. Qed.
+
+Lemma wf_local_app_renaming P Σ Γ Δ :
+  All_local_env (lift_typing (fun (Σ : global_env_ext) (Γ' : context) (t T : term) =>
+    forall P (Δ : PCUICEnvironment.context) (f : nat -> nat),
+    renaming (shiftnP #|Γ ,,, Γ'| P) Σ Δ (Γ ,,, Γ') f -> Σ ;;; Δ |- rename f t : rename f T) Σ)
+    Δ ->
+  forall Δ' f,
+  renaming (shiftnP #|Γ| P) Σ Δ' Γ f ->
+  wf_local Σ (Δ' ,,, rename_context f Δ).
+Proof.
+  intros. destruct X0.
+  induction X.
+  - apply a.
+  - simpl. destruct t0 as [s Hs].
+    rewrite rename_context_snoc /=. constructor; auto.
+    red. simpl. exists s.
+    eapply (Hs P (Δ' ,,, rename_context f Γ0) (shiftn #|Γ0| f)).
+    split => //.
+    eapply urenaming_ext.
+    { len. now rewrite -shiftnP_add. }
+    { reflexivity. } now eapply urenaming_context.
+  - destruct t0 as [s Hs]. red in t1.
+    rewrite rename_context_snoc /=. constructor; auto.
+    * red. exists s.
+      apply (Hs P (Δ' ,,, rename_context f Γ0) (shiftn #|Γ0| f)).
+      split => //.
+      eapply urenaming_ext.
+      { len; now rewrite -shiftnP_add. }
+      { reflexivity. } now eapply urenaming_context.
+    * red. apply (t1 P). split => //.
+      eapply urenaming_ext.
+      { len; now rewrite -shiftnP_add. }
+      { reflexivity. } now eapply urenaming_context.
+Qed.
+
+Lemma rename_decompose_prod_assum f Γ t :
+    decompose_prod_assum (rename_context f Γ) (rename (shiftn #|Γ| f) t)
+    = let '(Γ, t) := decompose_prod_assum Γ t in (rename_context f Γ, rename (shiftn #|Γ| f) t).
+Proof.
+  induction t in Γ |- *. all: try reflexivity.
+  - specialize (IHt2 (Γ ,, vass na t1)).
+    rewrite rename_context_snoc /= in IHt2.
+    simpl. now rewrite shiftn_add IHt2.
+  - specialize (IHt3 (Γ ,, vdef na t1 t2)).
+    rewrite rename_context_snoc /= in IHt3.
+    simpl. now rewrite shiftn_add IHt3.
+Qed.
+
+Lemma rename_app_context f Γ Δ :
+  rename_context f (Γ ,,, Δ) =
+  rename_context f Γ ,,, rename_context (shiftn #|Γ| f) Δ.
+Proof.
+  rewrite /rename_context fold_context_k_app /app_context. f_equal.
+  apply fold_context_k_ext. intros i x. now rewrite shiftn_add.
+Qed.
+
+Lemma rename_smash_context f Γ Δ :
+  rename_context f (smash_context Γ Δ) =
+  smash_context (rename_context (shiftn #|Δ| f) Γ) (rename_context f Δ).
+Proof.
+  induction Δ as [|[na [b|] ty] Δ] in Γ |- *; simpl; auto;
+    rewrite ?shiftn0 // ?rename_context_snoc IHΔ /=; len.
+  - f_equal. now rewrite rename_context_subst /= shiftn_add.
+  - f_equal. rewrite rename_app_context /map_decl /= /app_context.
+    f_equal.
+    * now rewrite shiftn_add.
+    * rewrite /rename_context fold_context_k_tip /map_decl /=. do 2 f_equal.
+      now rewrite shiftn0.
+Qed.
+
+Lemma nth_error_rename_context f Γ n :
+  nth_error (rename_context f Γ) n =
+  option_map (map_decl (rename (shiftn (#|Γ| - S n) f))) (nth_error Γ n).
+Proof.
+  induction Γ in n |- *; intros.
+  - simpl. unfold rename_context, fold_context_k; simpl; rewrite nth_error_nil. easy.
+  - simpl. destruct n; rewrite rename_context_snoc.
+    + simpl. lia_f_equal.
+    + simpl. rewrite IHΓ; simpl in *. 
+      assert (e : #|Γ| - S n = S #|Γ| - S (S n)). { lia. }
+      rewrite e. reflexivity.
+Qed.
+
+Lemma rename_check_one_fix f (mfix : mfixpoint term) d x :
+  check_one_fix d = Some x ->
+  check_one_fix (map_def (rename f) (rename (shiftn #|mfix| f)) d) = Some x.
+Proof.
+  destruct d; simpl.
+  move: (rename_decompose_prod_assum f [] dtype).
+  rewrite shiftn0. intros ->.
+  destruct decompose_prod_assum.
+  rewrite -(rename_smash_context f []).
+  destruct nth_error eqn:hnth => //.
+  pose proof (nth_error_Some_length hnth). len in H.
+  simpl in H.
+  destruct (nth_error (List.rev (rename_context _ _)) _) eqn:hnth'.
+  2:{ eapply nth_error_None in hnth'. len in hnth'. simpl in hnth'. lia. }
+  rewrite nth_error_rev_inv in hnth; len; auto.
+  len in hnth. simpl in hnth.
+  rewrite nth_error_rev_inv in hnth'; len; auto.
+  len in hnth'. simpl in hnth'.
+  rewrite nth_error_rename_context /= hnth /= in hnth'. noconf hnth'.
+  simpl.
+  destruct decompose_app eqn:da. len.
+  destruct t0 => /= //.
+  eapply decompose_app_inv in da. rewrite da.
+  rewrite rename_mkApps. simpl. rewrite decompose_app_mkApps //.
+Qed.
+
+Lemma rename_check_one_cofix f (mfix : mfixpoint term) d x :
+  check_one_cofix d = Some x ->
+  check_one_cofix (map_def (rename f) (rename (shiftn #|mfix| f)) d) = Some x.
+Proof.
+  destruct d; simpl.
+  move: (rename_decompose_prod_assum f [] dtype).
+  rewrite shiftn0. intros ->.
+  destruct decompose_prod_assum.
+  destruct decompose_app eqn:da.
+  destruct t0 => /= //.
+  eapply decompose_app_inv in da. rewrite da /=.
+  rewrite rename_mkApps. simpl. rewrite decompose_app_mkApps //.
+Qed.
+
+Lemma rename_wf_fixpoint Σ f mfix :
+  wf_fixpoint Σ mfix ->
+  wf_fixpoint Σ (map (map_def (rename f) (rename (shiftn #|mfix| f))) mfix).
+Proof.
+  unfold wf_fixpoint.
+  rewrite map_map_compose.
+  destruct (map_option_out (map check_one_fix mfix)) as [[]|] eqn:hmap => //.
+  eapply map_option_out_impl in hmap.
+  2:{ intros x y. apply (rename_check_one_fix f mfix). }
+  now rewrite hmap.
+Qed.
+
+Lemma rename_wf_cofixpoint Σ f mfix :
+  wf_cofixpoint Σ mfix ->
+  wf_cofixpoint Σ (map (map_def (rename f) (rename (shiftn #|mfix| f))) mfix).
+Proof.
+  rewrite /wf_cofixpoint map_map_compose.
+  destruct (map_option_out (map check_one_cofix mfix)) as [[]|] eqn:hmap => //.
+  eapply map_option_out_impl in hmap.
+  2:{ intros x y. apply (rename_check_one_cofix f mfix). }
+  now rewrite hmap.
+Qed.
+
+Lemma rename_subst_telescope f s Γ :
+  rename_telescope f (subst_telescope s 0 Γ) =
+  subst_telescope (map (rename f) s) 0
+    (rename_telescope (shiftn #|s| f) Γ).
+Proof.
+  rewrite /rename_telescope /subst_telescope.
+  rewrite !mapi_compose. apply mapi_ext => k' d.
+  rewrite !compose_map_decl; apply map_decl_ext => t'.
+  now rewrite Nat.add_0_r rename_subst.
+Qed.
+
+Instance rename_telescope_ext : Proper (`=1` ==> `=1`) rename_telescope.
+Proof.
+  intros f g Hfg Γ.
+  rewrite /rename_telescope. apply mapi_ext => n x.
+  now rewrite Hfg.
+Qed.
+
+Lemma rename_telescope_shiftn0 f Γ : rename_telescope (shiftn 0 f) Γ = rename_telescope f Γ.
+Proof. now sigma. Qed.
+
+Lemma rename_telescope_cons f d Γ :
+  rename_telescope f (d :: Γ) = rename_decl f d :: rename_telescope (shiftn 1 f) Γ.
+Proof.
+  rewrite /rename_telescope mapi_cons /rename_decl.
+  f_equal; sigma => //.
+  apply mapi_ext => i x. now rewrite shiftn_add Nat.add_1_r.
+Qed.
+
+Hint Rewrite <- Upn_ren : sigma.
+
+(** For an unconditional renaming defined on all variables in the source context *)
+Lemma typing_rename_prop : env_prop
+  (fun Σ Γ t A =>
+    forall P Δ f,
+    renaming (shiftnP #|Γ| P) Σ Δ Γ f ->
+    Σ ;;; Δ |- rename f t : rename f A)
+   (fun Σ Γ =>
+    wf_local Σ Γ ×
+   All_local_env
+   (lift_typing (fun (Σ : global_env_ext) (Γ : context) (t T : term)
+    =>
+    forall P (Δ : PCUICEnvironment.context) (f : nat -> nat),
+    renaming (shiftnP #|Γ| P) Σ Δ Γ f ->
+    Σ;;; Δ |- rename f t : rename f T) Σ) Γ).
+Proof.
+  apply typing_ind_env.
+
+  - intros Σ wfΣ Γ wfΓ HΓ. split; auto.
+    induction HΓ; constructor; firstorder eauto.
+
+  - intros Σ wfΣ Γ wfΓ n decl isdecl ihΓ P Δ f hf.
+    simpl in *.
+    eapply hf in isdecl as h => //.
+    2:{ rewrite /shiftnP. eapply nth_error_Some_length in isdecl. now nat_compare_specs. }
+    destruct h as [decl' [isdecl' [? [h1 h2]]]].
+    rewrite lift0_rename rename_compose h1 -lift0_rename.
+    econstructor. all: auto. apply hf.
+
+  - intros Σ wfΣ Γ wfΓ l X H0 P Δ f [hΔ hf].
+    simpl. constructor. all: auto.
+
+  - intros Σ wfΣ Γ wfΓ na A B s1 s2 X hA ihA hB ihB P Δ f hf.
+    rewrite /=. econstructor.
+    + eapply ihA; eauto.
+    + eapply ihB; eauto.
+      simpl.
+      eapply renaming_extP. { now rewrite -(shiftnP_add 1). }
+      eapply renaming_vass. 2: eauto.
+      constructor.
+      * destruct hf as [hΔ hf]. auto.
+      * simpl. exists s1. eapply ihA; eauto.
+  - intros Σ wfΣ Γ wfΓ na A t s1 B X hA ihA ht iht P Δ f hf.
+    simpl.
+     (* /andP [_ havB]. *)
+    simpl. econstructor.
+    + eapply ihA; eauto.
+    + eapply iht; eauto; simpl.
+      eapply renaming_extP. { now rewrite -(shiftnP_add 1). }
+      eapply renaming_vass. 2: eauto.
+      constructor.
+      * destruct hf as [hΔ hf]. auto.
+      * simpl. exists s1. eapply ihA; eauto.
+  - intros Σ wfΣ Γ wfΓ na b B t s1 A X hB ihB hb ihb ht iht P Δ f hf.
+    simpl. econstructor.
+    + eapply ihB; tea.
+    + eapply ihb; tea.
+    + eapply iht; tea.
+      eapply renaming_extP. { now rewrite -(shiftnP_add 1). }
+      eapply renaming_vdef. 2: eauto.
+      constructor.
+      * destruct hf. assumption.
+      * simpl. eexists. eapply ihB; tea.
+      * simpl. eapply ihb; tea.
+  - intros Σ wfΣ Γ wfΓ t na A B s u X hty ihty ht iht hu ihu P Δ f hf.
+    simpl. eapply meta_conv.
+    + eapply type_App.
+      * simpl in ihty. eapply ihty; tea.
+      * simpl in iht. eapply iht. eassumption.
+      * eapply ihu. eassumption.
+    + autorewrite with sigma. rewrite !subst1_inst. sigma.
+      eapply inst_ext => i.
+      unfold subst_cons, ren, shiftn, subst_compose. simpl.
+      destruct i.
+      * simpl. reflexivity.
+      * simpl. replace (i - 0) with i by lia.
+        reflexivity.
+  - intros Σ wfΣ Γ wfΓ cst u decl X X0 isdecl hconst P Δ f hf.
+    simpl. eapply meta_conv.
+    + constructor. all: eauto. apply hf.
+    + rewrite rename_subst_instance. f_equal.
+      rewrite rename_closed. 2: auto.
+      eapply declared_constant_closed_type. all: eauto.
+  - intros Σ wfΣ Γ wfΓ ind u mdecl idecl isdecl X X0 hconst P Δ σ hf.
+    simpl. eapply meta_conv.
+    + econstructor. all: eauto. apply hf.
+    + rewrite rename_subst_instance. f_equal.
+      rewrite rename_closed. 2: auto.
+      eapply declared_inductive_closed_type. all: eauto.
+  - intros Σ wfΣ Γ wfΓ ind i u mdecl idecl cdecl isdecl X X0 hconst P Δ f hf.
+    simpl. eapply meta_conv.
+    + econstructor. all: eauto. apply hf.
+    + rewrite rename_closed. 2: reflexivity.
+      eapply declared_constructor_closed_type. all: eauto.
+  - intros Σ wfΣ Γ wfΓ ci p c brs indices ps mdecl idecl isdecl HΣ.
+    intros [_ IHΔ] ci_npar eqpctx predctx wfp cup wfpctx Hpret IHpret [_ IHpredctx] isallowed.
+    intros Hcxti IHctxi Hc IHc iscof ptm wfbrs Hbrs P Δ f Hf.
+    simpl.
+    rewrite rename_mkApps.
+    rewrite map_app. simpl.
+    rewrite /ptm. rewrite rename_it_mkLambda_or_LetIn.
+    relativize #|predctx|.
+    * erewrite rename_predicate_preturn.
+      rewrite rename_case_predicate_context //.
+      eapply type_Case; eauto; tea; rewrite - ?rename_case_predicate_context.
+      all:tea.
+      + now eapply rename_wf_predicate.
+      + simpl. eauto.
+        apply All_local_env_app_inv in IHpredctx as [].
+        eapply wf_local_app_renaming; eauto. apply a0.
+      + simpl. eapply IHpret.
+        split.
+        ++ apply All_local_env_app_inv in IHpredctx as [].
+          eapply wf_local_app_renaming; eauto. apply a0.
+        ++ rewrite /predctx.
+           eapply urenaming_ext.
+           { len. now rewrite -shiftnP_add. }
+           { reflexivity. }
+          relativize #|pcontext p|; [eapply urenaming_context|].
+          { apply Hf. }
+          now rewrite case_predicate_context_length.
+      + revert IHctxi.
+        rewrite /= /id -map_app.
+        rewrite -{2}[subst_instance _ _](rename_closedn_ctx f 0).
+        { pose proof (declared_inductive_closed_pars_indices isdecl).
+          now rewrite closedn_subst_instance_context. }
+        rewrite rename_context_telescope.
+        rewrite rename_telescope_shiftn0.
+        clear -P Δ f Hf.
+        induction 1.
+        { constructor; auto. }
+        { simpl. rewrite rename_telescope_cons.
+          constructor; cbn; eauto.
+          now rewrite rename_subst_telescope /= in IHIHctxi. }
+        { simpl. rewrite rename_telescope_cons.
+          constructor; cbn; eauto.
+          now rewrite rename_subst_telescope /= in IHIHctxi. }
+      + simpl. unfold id.
+        specialize (IHc _ _ _ Hf).
+        now rewrite rename_mkApps map_app in IHc.
+      + now eapply rename_wf_branches.
+      + eapply Forall2_All2 in wfbrs.
+        eapply All2i_All2_mix_left in Hbrs; eauto.
+        eapply All2i_nth_hyp in Hbrs.
+        eapply All2i_map_right, (All2i_impl Hbrs) => i cdecl br.
+        set (brctxty := case_branch_type _ _ _ _ _ _ _ _).
+        move=> [Hnth [wfbr [eqbctx [[wfbctx IHbctx] [Hbod [IHbod [Hbty IHbty]]]]]]].
+        rewrite -(rename_closed_constructor_body mdecl cdecl f).
+        { eapply (declared_constructor_closed (c:=(ci.(ci_ind),i))); eauto.
+          split; eauto. }
+        split; auto.
+        { simpl. rewrite -rename_cstr_branch_context //.
+          1:eapply (declared_inductive_closed_params isdecl).
+          rewrite rename_closedn_ctx //.
+          eapply closed_cstr_branch_context. split; tea. }
+        cbn -[case_branch_type].
+        rewrite case_branch_type_fst.
+        rewrite -rename_case_branch_context_gen //.
+        2-3:len.
+        1:exact (declared_inductive_closed_params isdecl).
+        1:rewrite (wf_branch_length wfbr) //.
+        1:rewrite (wf_predicate_length_pars wfp).
+        1:now rewrite (declared_minductive_ind_npars isdecl).
+        set (brctx' := rename_context f _).
+        assert (wf_local Σ (Δ ,,, brctx')).
+        { apply All_local_env_app_inv in IHbctx as [].
+          eapply wf_local_app_renaming; tea. simpl. apply a0. }
+        split => //.
+        rewrite rename_case_predicate_context // rename_case_branch_type //.
+        split.
+        { eapply IHbod => //.
+          split => //.
+          * eapply urenaming_ext.
+          { now rewrite app_context_length -shiftnP_add. }
+          { reflexivity. }
+          relativize #|bcontext br|; [eapply urenaming_context|].
+          1:apply Hf. rewrite /brctxty case_branch_type_fst case_branch_context_length //. }
+        { eapply IHbty. split=> //.
+          rewrite /brctx' case_branch_type_fst.
+          rewrite (wf_branch_length wfbr).
+          eapply urenaming_ext.
+          { now rewrite app_context_length -shiftnP_add. }
+          { reflexivity. }
+          rewrite -(wf_branch_length wfbr).
+          rewrite -/(rename_context f _).
+          relativize #|bcontext br|; [eapply urenaming_context, Hf|len].
+          now rewrite case_branch_context_length. }
+    * rewrite /predctx case_predicate_context_length //.
+  - intros Σ wfΣ Γ wfΓ p c u mdecl idecl cdecl pdecl isdecl args X X0 hc ihc e ty
+           P Δ f hf.
+    simpl. eapply meta_conv.
+    + econstructor.
+      * eassumption.
+      * eapply meta_conv.
+        -- eapply ihc; tea.
+        -- rewrite rename_mkApps. simpl. reflexivity.
+      * rewrite map_length. assumption.
+    + rewrite rename_subst0. simpl. rewrite map_rev. f_equal.
+      rewrite rename_subst_instance. f_equal.
+      rewrite rename_closedn. 2: reflexivity.
+      eapply declared_projection_closed_type in isdecl.
+      rewrite List.rev_length. rewrite e. assumption.
+
+  - intros Σ wfΣ Γ wfΓ mfix n decl types H1 hdecl [_ X] ihmfixt ihmfixb wffix P Δ f hf.
+    apply All_local_env_app_inv in X as [_ X].
+    eapply wf_local_app_renaming in X; tea.
+    simpl. eapply meta_conv.
+    + eapply type_Fix.
+      * destruct hf; eapply fix_guard_rename; eauto.
+      * rewrite nth_error_map. rewrite hdecl. simpl. reflexivity.
+      * apply hf.
+      * apply All_map, (All_impl ihmfixt).
+        intros x [s [Hs IHs]].
+        exists s. now eapply IHs.
+      * apply All_map, (All_impl ihmfixb).
+        intros x [Hb IHb].
+        destruct x as [na ty bo rarg]. simpl in *.
+        rewrite rename_fix_context.
+        eapply meta_conv.
+        ++ apply (IHb P (Δ ,,, rename_context f types) (shiftn #|mfix| f)).
+          split; auto. subst types. rewrite -(fix_context_length mfix).
+          eapply urenaming_ext.
+          { now rewrite app_context_length -shiftnP_add. }
+          { reflexivity. }
+          apply urenaming_context; auto. apply hf.
+        ++ len. now sigma.
+      * now eapply rename_wf_fixpoint.
+    + reflexivity.
+
+  - intros Σ wfΣ Γ wfΓ mfix n decl types guard hdecl [_ X] ihmfixt ihmfixb wfcofix P Δ f hf.
+    apply All_local_env_app_inv in X as [_ X].
+    eapply wf_local_app_renaming in X; eauto.
+    simpl. eapply meta_conv.
+    + eapply type_CoFix; auto.
+      * destruct hf; eapply cofix_guard_rename; eauto.
+      * rewrite nth_error_map. rewrite hdecl. simpl. reflexivity.
+      * apply hf.
+      * apply All_map, (All_impl ihmfixt).
+        intros x [s [Hs IHs]].
+        exists s. now eapply IHs.
+      * apply All_map, (All_impl ihmfixb).
+        intros x [Hb IHb].
+        destruct x as [na ty bo rarg]. simpl in *.
+        rewrite rename_fix_context.
+        eapply meta_conv.
+        ++ apply (IHb P (Δ ,,, rename_context f types) (shiftn #|mfix| f)).
+            split; auto. subst types. rewrite -(fix_context_length mfix).
+            eapply urenaming_ext.
+            { now rewrite app_context_length -shiftnP_add. }
+            { reflexivity. }
+            apply urenaming_context; auto. apply hf.
+        ++ len. now sigma.
+      * now eapply rename_wf_cofixpoint.
+    + reflexivity.
+
+  - intros Σ wfΣ Γ wfΓ t A B X hwf ht iht htB ihB cum P Δ f hf.
+    eapply type_Cumul.
+    + eapply iht; tea.
+    + eapply ihB; tea.
+    + eapply cumulSpec_renameP. all: try eassumption.
+      * apply hf.
+      * pose proof (type_closed ht).
+        now eapply closedn_on_free_vars in H.
+      * pose proof (subject_closed htB).
+        now eapply closedn_on_free_vars in H.
+      * pose proof (closed_ctx_on_free_vars P _ (closed_wf_local _ (typing_wf_local ht))).
+        rewrite -{2}(app_context_nil_l Γ).
+        rewrite on_ctx_free_vars_extend //.
+Qed.
+
+Lemma typing_rename_P {P Σ Γ Δ f t A} {wfΣ : wf Σ.1} :
+  renaming (shiftnP #|Γ| P) Σ Δ Γ f ->
+  Σ ;;; Γ |- t : A ->
+  Σ ;;; Δ |- rename f t : rename f A.
+Proof.
+  intros hf h.
+  revert Σ wfΣ Γ t A h P Δ f hf.
+  apply typing_rename_prop.
+Qed.
+
+Lemma typing_rename {Σ Γ Δ f t A} {wfΣ : wf Σ.1} :
+  renaming (closedP #|Γ| xpredT) Σ Δ Γ f ->
+  Σ ;;; Γ |- t : A ->
+  Σ ;;; Δ |- rename f t : rename f A.
+Proof.
+  intros hf h.
+  eapply (typing_rename_P (P:=fun _ => false)) ; eauto.
+Qed.
+
+End Renaming.
